Organise process operations components

src/dafny/beacon/Helpers.dfy
@@ -44,6 +44,480 @@ module BeaconHelpers {
     import opened AttestationsTypes
     import opened Validators
     
+     /**
+     * Extract a validator from a single deposit.
+     *
+     *  @param  d       A single deposit.
+     *  @returns        A validator created from the deposit information
+     *
+     *  @note           The `effective_balance` is not an active field in the current model but the code
+     *                  to set this field is included as a comment for future reference.
+     */
+    function method get_validator_from_deposit(d: Deposit): Validator
+        ensures get_validator_from_deposit(d).effective_balance <= MAX_EFFECTIVE_BALANCE as Gwei
+    {
+        var amount := d.data.amount; 
+        var effective_balance := min((amount as nat- amount as nat % EFFECTIVE_BALANCE_INCREMENT as nat) as nat, MAX_EFFECTIVE_BALANCE as nat);
+
+        Validator(d.data.pubkey, effective_balance as Gwei, false, FAR_FUTURE_EPOCH, FAR_FUTURE_EPOCH, FAR_FUTURE_EPOCH, FAR_FUTURE_EPOCH)
+    }
+
+    /**
+     *  Append a new validator
+     */
+    function method validator_append(sv: ListOfValidators, v: Validator): ListOfValidators
+        requires |sv| + 1 <= VALIDATOR_REGISTRY_LIMIT as int
+    {
+        sv + [v]
+    }
+    /**
+     *  Append a new balance entry
+     */
+    function method balance_append(sb: ListOfBalances, b: Gwei): ListOfBalances
+        requires |sb| + 1 <= VALIDATOR_REGISTRY_LIMIT as int
+    {
+        sb + [b]
+    }
+
+     /**
+     *  Get the index of a validator. 
+     *
+     *  @notes  Helper function as no alternative indexing functionality available.
+     *
+     */
+    function method get_validator_index(pk: seq<BLSPubkey>, pubkey: BLSPubkey) : ValidatorIndex
+        requires |pk| < VALIDATOR_REGISTRY_LIMIT as int
+        requires pubkey in pk
+        ensures get_validator_index(pk,pubkey) as int < |pk|
+        ensures pk[get_validator_index(pk,pubkey)] == pubkey
+        decreases pk
+    {
+        if pk[0] == pubkey then 0 as ValidatorIndex
+        else 1 + get_validator_index(pk[1..], pubkey)
+        // alternative reverse form
+        //if pk[|pk|-1] == pubkey then (|pk|-1) as ValidatorIndex
+        //else get_validator_index(pk[..|pk|-1], pubkey)
+
+    }
+
+
+    // Beacon State Mutators
+
+/** increase_balance
+     *  Increase the validator balance at index ``index`` by ``delta``.
+     *
+     *  @notes  The datatype Gwei has temporarily been changed from uint64 to nat so as to simplify the
+     *          properties required to process a deposit. Hence a further requires will be needed to prevent
+     *          overflow once this temporary simplification is removed.
+     *  
+     **/
+    // function method increase_balance(s: BeaconState, index: ValidatorIndex, delta: Gwei): BeaconState 
+    //     requires index as int < |s.balances| 
+    //     requires s.balances[index] as int + delta as int < 0x10000000000000000
+    //     ensures |s.balances| == |increase_balance(s,index,delta).balances|
+    //     ensures increase_balance(s,index,delta).balances[index] == s.balances[index] + delta
+    // {
+    //     s.(
+    //         balances := s.balances[index as int := (s.balances[index] + delta)]
+    //     )
+    // }
+    
+    /** increase_balance
+     *  Increase the validator balance at index ``index`` by ``delta``.
+     *  
+     **/
+    function method increase_balance(s: BeaconState, index: ValidatorIndex, delta: Gwei): BeaconState 
+        requires index as int < |s.balances| 
+        requires s.balances[index] as int + delta as int < 0x10000000000000000
+        ensures |s.balances| == |increase_balance(s,index,delta).balances|
+        ensures increase_balance(s,index,delta).balances[index] == s.balances[index] + delta
+    {
+        s.(
+            balances := s.balances[index as int := (s.balances[index] + delta)]
+        )
+    }
+
+    /** decrease_balance
+     *  Decrease the validator balance at index ``index`` by ``delta``.
+     *
+     **/
+    function method decrease_balance(s: BeaconState, index: ValidatorIndex, delta: Gwei): BeaconState 
+        requires index as int < |s.balances| 
+        ensures |s.balances| == |decrease_balance(s,index,delta).balances|
+        ensures if s.balances[index] > delta then decrease_balance(s,index,delta).balances[index] == s.balances[index] - delta
+                else decrease_balance(s,index,delta).balances[index] == 0
+        ensures s.validators == decrease_balance(s,index,delta).validators
+    {
+        if s.balances[index] > delta then
+            s.(
+                balances := s.balances[index as int := (s.balances[index] - delta)]
+            )
+        else
+            s.(
+                balances := s.balances[index as int := 0]
+            )
+    }
+
+    function method sorted_intersection(a : seq<ValidatorIndex>, b: seq<ValidatorIndex>): seq<uint64>
+        requires forall i,j :: 0 <= i < j < |a| ==> a[i] < a[j]
+        requires forall i,j :: 0 <= i < j < |b| ==> b[i] < b[j]
+        ensures forall i,j :: 0 <= i < j < |sorted_intersection(a,b)| ==> sorted_intersection(a,b)[i] < sorted_intersection(a,b)[j]
+        ensures forall i :: 0 <= i < |sorted_intersection(a,b)| ==> sorted_intersection(a,b)[i] as ValidatorIndex in a &&
+                                                                    sorted_intersection(a,b)[i] as ValidatorIndex in b
+        ensures sorted_intersection(a,b) == sorted_intersection_fn(a,b)
+    {
+        if |a| == 0 then []
+        else (if a[0] in b then [a[0] as uint64] else []) + sorted_intersection(a[1..], b)
+    }
+
+        
+    
+    /** initiate_validator_exit
+     *  
+     *  Initiate the exit of the validator with index ``index``.
+     *
+     */
+    function method initiate_validator_exit(s: BeaconState, index: ValidatorIndex) : BeaconState
+        requires |s.validators| == |s.balances|
+        requires index as int < |s.validators| 
+        //requires s.validators[index].exitEpoch == FAR_FUTURE_EPOCH
+
+        ensures |s.validators| == |initiate_validator_exit(s,index).validators|
+        ensures |initiate_validator_exit(s,index).validators| == |initiate_validator_exit(s,index).balances|
+        ensures initiate_validator_exit(s,index).validators[index].exitEpoch > get_current_epoch(s) + MAX_SEED_LOOKAHEAD
+                || initiate_validator_exit(s,index).validators[index].exitEpoch == s.validators[index].exitEpoch
+        ensures forall i :: (0 <= i < |s.validators|) && (i != index as int) ==> 
+                initiate_validator_exit(s,index).validators[i].exitEpoch == s.validators[i].exitEpoch
+        ensures initiate_validator_exit(s,index).validators[index].exitEpoch < FAR_FUTURE_EPOCH
+    {
+        // # Return if validator already initiated exit
+        // validator = state.validators[index]
+        if s.validators[index].exitEpoch != FAR_FUTURE_EPOCH then
+            s
+        else 
+        //     return
+        //assert s.validators[index].exitEpoch == FAR_FUTURE_EPOCH;
+        
+        // # Compute exit queue epoch
+        // exit_epochs = [v.exit_epoch for v in state.validators if v.exit_epoch != FAR_FUTURE_EPOCH]
+        var exit_epochs := get_exit_epochs(s.validators);
+        
+        // exit_queue_epoch = max(exit_epochs + [compute_activation_exit_epoch(get_current_epoch(state))])
+        var exit_queue_epoch := max_epoch(exit_epochs + [compute_activation_exit_epoch(get_current_epoch(s))]);
+
+        assert compute_activation_exit_epoch(get_current_epoch(s)) > get_current_epoch(s) + MAX_SEED_LOOKAHEAD;
+        assert compute_activation_exit_epoch(get_current_epoch(s)) in exit_epochs + [compute_activation_exit_epoch(get_current_epoch(s))];
+        assert max_epoch(exit_epochs + [compute_activation_exit_epoch(get_current_epoch(s))]) >= compute_activation_exit_epoch(get_current_epoch(s));
+        assert exit_queue_epoch > get_current_epoch(s) + MAX_SEED_LOOKAHEAD;
+
+        // exit_queue_churn = len([v for v in state.validators if v.exit_epoch == exit_queue_epoch])
+        var exit_queue_churn := |get_queue_churn(s.validators, exit_queue_epoch)|;
+        var validator_churn_limit := get_validator_churn_limit(s);
+
+        // if exit_queue_churn >= get_validator_churn_limit(state):
+        //     exit_queue_epoch += Epoch(1)
+
+        // # Set validator exit epoch and withdrawable epoch
+        // validator.exit_epoch = exit_queue_epoch
+        // validator.withdrawable_epoch = Epoch(validator.exit_epoch + MIN_VALIDATOR_WITHDRAWABILITY_DELAY)
+
+        assume exit_queue_epoch as int + 1 + MIN_VALIDATOR_WITHDRAWABILITY_DELAY as nat < 0x10000000000000000; 
+
+        if exit_queue_churn  >= get_validator_churn_limit(s) as nat then 
+            s.(validators := s.validators[index as int := s.validators[index].(exitEpoch := exit_queue_epoch + 1 as Epoch,
+                                                            withdrawable_epoch := (exit_queue_epoch as nat + 1 + MIN_VALIDATOR_WITHDRAWABILITY_DELAY as nat) as Epoch)])
+        else
+            s.(validators := s.validators[index as int := s.validators[index].(exitEpoch := exit_queue_epoch,
+                                                            withdrawable_epoch := (exit_queue_epoch as nat + MIN_VALIDATOR_WITHDRAWABILITY_DELAY as nat) as Epoch)])
+    }
+
+
+        /** slash_validator
+     *  
+     *  Slash the validator with index ``slashed_index``.
+     */
+    function method slash_validator(s: BeaconState, slashed_index: ValidatorIndex, whistleblower_index: ValidatorIndex): BeaconState
+        requires slashed_index as int < |s.validators| 
+        requires whistleblower_index as int < |s.validators| 
+        requires |s.validators| == |s.balances|
+        //requires s.validators[slashed_index].exitEpoch == FAR_FUTURE_EPOCH
+        requires |get_active_validator_indices(s.validators, get_current_epoch(s))| > 0
+        //ensures |get_active_validator_indices(slash_validator(s,slashed_index,whistleblower_index).validators, get_current_epoch(s))| > 0
+        ensures slash_validator(s, slashed_index, whistleblower_index).slot == s.slot
+    {
+        var epoch : Epoch := get_current_epoch(s);
+        var proposer_index := get_beacon_proposer_index(s);
+
+        var s' := initiate_validator_exit(s, slashed_index); // only validator exitEpoch & withdrawable_epoch fields possibly changed
+
+        assert |s.balances| == |s'.balances|;
+        assert |s'.balances| == |s'.validators|;
+        assert get_current_epoch(s) == get_current_epoch(s');
+        
+        //assert initiate_validator_exit(s,slashed_index).validators[slashed_index].exitEpoch > get_current_epoch(s) + MAX_SEED_LOOKAHEAD;
+        assert forall i :: (0 <= i < |s.validators|) && (i != slashed_index as int) ==> 
+                initiate_validator_exit(s,slashed_index).validators[i].exitEpoch == s.validators[i].exitEpoch;
+        
+        //assert s'.validators[slashed_index].exitEpoch > get_current_epoch(s) + MAX_SEED_LOOKAHEAD;
+        assert forall i :: (0 <= i < |s.validators|) && (i != slashed_index as int) ==> 
+                s'.validators[i].exitEpoch == s.validators[i].exitEpoch;
+        
+        assert forall i :: (0 <= i < |s'.validators|) ==> 
+                is_active_validator(s.validators[i], get_current_epoch(s)) == is_active_validator(s'.validators[i], get_current_epoch(s'));
+
+        initiateValidatorExitPreservesActivateValidators(s.validators, s'.validators,  get_current_epoch(s'));
+        assert get_active_validator_indices(s'.validators, get_current_epoch(s')) == get_active_validator_indices(s.validators, get_current_epoch(s));
+        assert |get_active_validator_indices(s'.validators, get_current_epoch(s'))| > 0;
+        
+        // NOTE:    steps reordered to suit Dafny function method output
+        //          order irrelevant as 'Apply proposer and whistleblower rewards' relies only on s'.validators[slashed_index].effective_balance
+
+        // # Apply proposer and whistleblower rewards
+        
+        // if whistleblower_index is None:
+        //     whistleblower_index = proposer_index
+        // Note: 'None' is not available in Dafny and so functions that call slash_validator will have this parameter set to proposer_index
+        
+        
+        // NOTE: there doesn't seem to be anything to check that the validator being slashed isn't the proposer of the block that contains the ps
+        // though it makes sense that a validator wouldn't proposer to slash itself!
+        // assert slashed_index != whistleblower_index;
+
+        var whistleblower_reward : Gwei := (s'.validators[slashed_index].effective_balance as int / WHISTLEBLOWER_REWARD_QUOTIENT as nat) as Gwei;
+        var proposer_reward := (whistleblower_reward as int / PROPOSER_REWARD_QUOTIENT as int) as Gwei;
+        var validator_penalty := (s'.validators[slashed_index].effective_balance as int / MIN_SLASHING_PENALTY_QUOTIENT as nat) as Gwei;
+
+        //s' := increase_balance(s', proposer_index, proposer_reward);
+        //s' := increase_balance(s', whistleblower_index, Gwei(whistleblower_reward - proposer_reward));
+        
+        //var validator := s'.validators[slashed_index];
+        // validator.slashed = True
+        // validator.withdrawable_epoch = max(validator.withdrawable_epoch, Epoch(epoch + EPOCHS_PER_SLASHINGS_VECTOR))
+        // state.slashings[epoch % EPOCHS_PER_SLASHINGS_VECTOR] += validator.effective_balance
+
+        assume (s'.slashings[epoch as int % EPOCHS_PER_SLASHINGS_VECTOR as nat] as int + s'.validators[slashed_index].effective_balance as int) < 0x10000000000000000;
+        assert slashed_index as int < |s'.balances|; 
+        assert proposer_index as int < |s'.balances|; 
+        assert whistleblower_index as int < |s'.balances|; 
+        assume s'.balances[proposer_index] as int + proposer_reward as int < 0x10000000000000000;
+        // Note: if proposer_index == whistleblower_index then the following assume statement is required rather than
+        // assume s'.balances[whistleblower_index] as int + (whistleblower_reward - proposer_reward) as int < 0x10000000000000000;
+        // The following assume statement covers both cases and will be replaced at a later date by functionality that
+        // takes into account the total amount of Eth available.
+        assume s'.balances[whistleblower_index] as int + whistleblower_reward  as int < 0x10000000000000000;
+
+        s'.(validators := s'.validators[slashed_index := s'.validators[slashed_index].(slashed := true,
+                                                            withdrawable_epoch := max(s'.validators[slashed_index].withdrawable_epoch as nat,(epoch as nat + EPOCHS_PER_SLASHINGS_VECTOR as nat)) as Epoch)],
+            slashings := s'.slashings[(epoch as int % EPOCHS_PER_SLASHINGS_VECTOR as nat) := s'.slashings[epoch as int % EPOCHS_PER_SLASHINGS_VECTOR as nat] + s'.validators[slashed_index].effective_balance],
+            balances := increase_balance(
+                            increase_balance(
+                                decrease_balance(s', slashed_index, validator_penalty), 
+                                proposer_index, 
+                                proposer_reward), 
+                            whistleblower_index, 
+                            (whistleblower_reward - proposer_reward)).balances)
+            
+        
+        // the triple nested mutation of balances is somewhat messy but for the moment it allows slashed_validator to remain as a function method 
+        //(rather than a method)
+
+    }
+
+    function method get_exit_epochs(sv: ListOfValidators) : seq<Epoch>
+        ensures forall i :: 0 <= i < |get_exit_epochs(sv)| ==> get_exit_epochs(sv)[i] < FAR_FUTURE_EPOCH
+    {
+        if |sv| == 0 
+            then []
+        else 
+            if sv[0].exitEpoch != FAR_FUTURE_EPOCH 
+                then [sv[0].exitEpoch] + get_exit_epochs(sv[1..])
+                else get_exit_epochs(sv[1..])
+    }
+
+    function method get_queue_churn(sv: ListOfValidators, exit_queue_epoch: Epoch) : seq<Validator>
+    {
+        if |sv| == 0 
+            then []
+        else 
+            if sv[0].exitEpoch == exit_queue_epoch 
+                then [sv[0]] + get_queue_churn(sv[1..], exit_queue_epoch)
+                else get_queue_churn(sv[1..], exit_queue_epoch)
+    }
+
+    // // Check if ``validator`` is active.
+    // predicate method is_active_validator(validator: Validator, epoch: Epoch)
+    // {
+    //     validator.activation_epoch <= epoch < validator.exitEpoch
+    // }
+
+    // // Return the sequence of active validator indices at ``epoch``.
+    // // function get_active_validator_indices(s: BeaconState, epoch: Epoch) : seq<ValidatorIndex>
+    // // NOTE: as BeaconState isn't modified and only validators field is accessed, the function is better suited to 
+    // //      using an input parameter of just the list of validators (rather than the entire state)
+    // function method get_active_validator_indices(sv: ListOfValidators, epoch: Epoch) : seq<ValidatorIndex>
+    //     ensures |get_active_validator_indices(sv,epoch)| <= |sv|
+    // {
+    //     //[ValidatorIndex(i) for i, v in enumerate(state.validators) if is_active_validator(v, epoch)]
+    //     if |sv| == 0 then []
+    //     else 
+    //         if is_active_validator(sv[|sv|-1], epoch) then get_active_validator_indices(sv[..|sv|-1], epoch) + [(|sv|-1) as ValidatorIndex]
+    //         else get_active_validator_indices(sv[..|sv|-1], epoch)
+    // }
+
+    //Return the validator churn limit for the current epoch.
+    function method get_validator_churn_limit(s: BeaconState) : uint64
+        //ensures MIN_PER_EPOCH_CHURN_LIMIT <= get_validator_churn_limit(s) <= 
+        //    (|get_active_validator_indices(s.validators, get_current_epoch(s))| as uint64/CHURN_LIMIT_QUOTIENT)  // i.e. at least 4
+    {
+        var active_validator_indices := get_active_validator_indices(s.validators, get_current_epoch(s));
+        max(MIN_PER_EPOCH_CHURN_LIMIT as nat, (|active_validator_indices| as uint64/CHURN_LIMIT_QUOTIENT) as nat) as uint64
+    }
+
+
+    function method max_epoch(se: seq<Epoch>): Epoch
+        requires |se| > 0
+        ensures forall i :: 0 <= i < |se| ==> max_epoch(se) >= se[i]
+        decreases se
+    {
+        if |se| == 1 then se[0]
+        else
+            if se[0] > max_epoch(se[1..]) then se[0]
+            else max_epoch(se[1..])
+    }
+    
+    // Return the epoch during which validator activations and exits initiated in ``epoch`` take effect.
+    function method compute_activation_exit_epoch(epoch: Epoch) : Epoch
+        requires epoch as int + 1 + MAX_SEED_LOOKAHEAD as int < 0x10000000000000000 
+        ensures compute_activation_exit_epoch(epoch) > epoch
+    {
+        epoch + 1 as Epoch + MAX_SEED_LOOKAHEAD as Epoch
+    }
+
+    //Return from ``indices`` a random index sampled by effective balance.
+    function method compute_proposer_index(state: BeaconState, indices: seq<ValidatorIndex>, seed: Bytes32) : ValidatorIndex
+        requires |indices| > 0
+    {
+        // assert len(indices) > 0
+
+        var MAX_RANDOM_BYTE := TWO_UP_8 - 1;
+        var i : uint64 := 0;
+        var total := |indices|;
+        //while true {
+        //     candidate_index = indices[compute_shuffled_index(i % total, total, seed)]
+        //     random_byte = hash(seed + uint_to_bytes(uint64(i // 32)))[i % 32]
+        //     effective_balance = state.validators[candidate_index].effective_balance
+        //     if effective_balance * MAX_RANDOM_BYTE >= MAX_EFFECTIVE_BALANCE * random_byte:
+        //         return candidate_index
+        //    i := i + 1;
+        //}
+        
+        
+        0 as ValidatorIndex // temporary return value
+    }
+
+    // Return the shuffled index corresponding to ``seed`` (and ``index_count``).
+    // Swap or not (https://link.springer.com/content/pdf/10.1007%2F978-3-642-32009-5_1.pdf)
+    // See the 'generalized domain' algorithm on page 3
+    function method compute_shuffled_index(index: uint64, index_count: uint64, seed: Bytes32): ValidatorIndex
+        requires index < index_count
+    {
+        // for current_round in range(SHUFFLE_ROUND_COUNT):
+        //     pivot = bytes_to_uint64(hash(seed + uint_to_bytes(uint8(current_round)))[0:8]) % index_count
+        //     flip = (pivot + index_count - index) % index_count
+        //     position = max(index, flip)
+        //     source = hash(
+        //         seed
+        //         + uint_to_bytes(uint8(current_round))
+        //         + uint_to_bytes(uint32(position // 256))
+        //     )
+        //     byte = uint8(source[(position % 256) // 8])
+        //     bit = (byte >> (position % 8)) % 2
+        //     index = flip if bit else index
+
+        // return index
+
+        0 as ValidatorIndex // temporary return value
+
+    }
+
+    //Return the beacon proposer index at the current slot.
+    function method get_beacon_proposer_index(state: BeaconState): ValidatorIndex
+        requires |get_active_validator_indices(state.validators, get_current_epoch(state))| > 0
+        //ensures is_active_validator(state.validators[get_beacon_proposer_index(state)], get_current_epoch(state))
+    {
+        var epoch := get_current_epoch(state);
+        var seed := hash(serialise(get_seed(state, epoch, DOMAIN_BEACON_PROPOSER)) + serialise(Uint64(state.slot as nat)));
+        var indices := get_active_validator_indices(state.validators, epoch);
+
+        compute_proposer_index(state, indices, seed)
+    }
+
+    // is_slashable_attestation_data
+    // Check if ``data_1`` and ``data_2`` are slashable according to Casper FFG rules.
+    predicate method is_slashable_attestation_data(data_1: AttestationData, data_2: AttestationData)
+    {
+        // Double vote
+        (data_1 != data_2 && data_1.target.epoch == data_2.target.epoch) ||
+        // Surround vote
+        (data_1.source.epoch < data_2.source.epoch && data_2.target.epoch < data_1.target.epoch)
+    }
+
+    predicate method is_valid_indexed_attestation(s: BeaconState, indexed_attestation: IndexedAttestation)
+    {
+        // Verify indices are sorted and unique
+        var indices := indexed_attestation.attesting_indices;
+        //if len(indices) == 0 or not indices == sorted(set(indices)):
+        if (|indices| == 0 || !is_attesting_indices_sorted_and_unique(indices))
+            then false
+        else 
+            true
+
+        // Verify aggregate signature, not implemented at this time
+
+        // pubkeys = [state.validators[i].pubkey for i in indices]
+        // domain = get_domain(state, DOMAIN_BEACON_ATTESTER, indexed_attestation.data.target.epoch)
+        // signing_root = compute_signing_root(indexed_attestation.data, domain)
+        // return bls.FastAggregateVerify(pubkeys, signing_root, indexed_attestation.signature)
+    }
+
+    predicate method is_attesting_indices_sorted_and_unique(indices: AttestingIndices)
+        requires |indices| > 0
+    {
+        forall i,j :: 0 <= i < j < |indices| ==> indices[i] < indices[j]
+    }
+
+    
+    /**
+     *  Collect pubkey in a list of validators.
+     *
+     *  @param  xv  A list of validators,
+     *  @returns    The sequence\list of keys helpd byt the validators in `xv`.
+     */
+    function method seqKeysInValidators(xv : seq<Validator>) : seq<BLSPubkey>
+        ensures |seqKeysInValidators(xv)| == |xv|
+        decreases xv
+    {
+        if |xv| == 0 then  
+            []
+        else 
+            [ xv[0].pubkey ] + seqKeysInValidators(xv[1..])
+    }
+
+    /**
+     *  Collect pubkey in a list of deposits.
+     *
+     *  @param  xd  A list of validators,
+     *  @returns    The sequence\list of keys held by the depositors in `xd`.
+     */
+    function method seqKeysInDeposits(xd : seq<Deposit>) : seq<BLSPubkey>
+        ensures |seqKeysInDeposits(xd)| == |xd|
+        decreases xd
+    {
+        if |xd| == 0 then  
+            []
+        else 
+            [ xd[0].data.pubkey ] + seqKeysInDeposits(xd[1..])
+    }
 
     
     /**
@@ -384,6 +858,11 @@ module BeaconHelpers {
 
 
     
+    // //Return the randao mix at a recent ``epoch``.
+    // function method get_randao_mix(state: BeaconState, epoch: Epoch): Bytes32
+    // {
+    //     state.randao_mixes[epoch % EPOCHS_PER_HISTORICAL_VECTOR as uint64]
+    // }
 
      //Return the randao mix at a recent ``epoch``.
     function method get_randao_mix(state: BeaconState, epoch: Epoch): Bytes32
@@ -391,6 +870,14 @@ module BeaconHelpers {
         state.randao_mixes[epoch % EPOCHS_PER_HISTORICAL_VECTOR as uint64]
     }
 
+    // // Return the seed at ``epoch``.
+    // function method get_seed(state: BeaconState, epoch: Epoch, domain_type: DomainType): Bytes32
+    //     requires epoch as int + EPOCHS_PER_HISTORICAL_VECTOR - MIN_SEED_LOOKAHEAD  - 1 < 0x10000000000000000
+    // {
+    //     var mix := get_randao_mix(state, (epoch as int + EPOCHS_PER_HISTORICAL_VECTOR - MIN_SEED_LOOKAHEAD - 1) as uint64);  // Avoid underflow
+    //     var sb := serialise(domain_type) + serialise(Uint64(epoch as nat)) + serialise(mix);
+    //     hash(sb)
+    // }
     // Return the seed at ``epoch``.
     function method get_seed(state: BeaconState, epoch: Epoch, domain_type: DomainType): Bytes32
         requires epoch as nat + EPOCHS_PER_HISTORICAL_VECTOR as nat - MIN_SEED_LOOKAHEAD as nat  - 1 < 0x10000000000000000
