src/dafny/beacon/Helpers.s.dfy
@@ -67,4 +67,50 @@ module BeaconHelperSpec {
             { xv[0].pubkey } + keysInValidators(xv[1..])
     }
 
+
+    function total_deposits(deposits: seq<Deposit>): nat
+    {
+        if |deposits| == 0 then 0
+        //else deposits[0].data.amount as nat + total_deposits(deposits[1..])
+        else total_deposits(deposits[..|deposits|-1]) + deposits[|deposits|-1].data.amount as nat
+    }
+
+    function total_balances(bal: seq<Gwei>): nat
+    {
+        if |bal| == 0 then 0
+        else bal[0] as nat + total_balances(bal[1..])
+    }
+
+    function get_VolExit_validator_indices(ve: seq<VoluntaryExit>): seq<int>
+        ensures |get_VolExit_validator_indices(ve)| == |ve|
+    {
+        if |ve| == 0 then []
+        else [ve[0].validator_index as int] + get_VolExit_validator_indices(ve[1..])
+    }
+
+    function get_PS_validator_indices(ps: seq<ProposerSlashing>): seq<int>
+        ensures |get_PS_validator_indices(ps)| == |ps|
+    {
+        if |ps| == 0 then []
+        else [ps[0].header_1.proposer_index as int] + get_PS_validator_indices(ps[1..])
+    }
+
+
+    function sorted_intersection_fn(a : seq<ValidatorIndex>, b: seq<ValidatorIndex>): seq<uint64>
+        requires forall i,j :: 0 <= i < j < |a| ==> a[i] < a[j]
+        requires forall i,j :: 0 <= i < j < |b| ==> b[i] < b[j]
+        ensures forall i,j :: 0 <= i < j < |sorted_intersection_fn(a,b)| ==> sorted_intersection_fn(a,b)[i] < sorted_intersection_fn(a,b)[j]
+        ensures forall i :: 0 <= i < |sorted_intersection_fn(a,b)| ==> sorted_intersection_fn(a,b)[i] as ValidatorIndex in a &&
+                                                                    sorted_intersection_fn(a,b)[i] as ValidatorIndex in b
+    {
+        if |a| == 0 then []
+        else (if a[0] in b then [a[0] as uint64] else []) + sorted_intersection_fn(a[1..], b)
+    }
+
+    predicate valid_state_indices(s: BeaconState, indices: seq<uint64>)
+    {
+        forall i :: 0 <= i < |indices| ==> indices[i] as int < |s.validators|
+    }
+    
+
 }
