src/dafny/beacon/statetransition/ProcessOperations.s.dfy
@@ -44,109 +44,119 @@ module ProcessOperationsSpec {
     import opened MathHelpers
     import opened SSZ
 
-/**
-     *  Collect pubkey in a list of validators.
-     *
-     *  @param  xv  A list of validators,
-     *  @returns    The sequence\list of keys helpd byt the validators in `xv`.
-     */
-    function method seqKeysInValidators(xv : seq<Validator>) : seq<BLSPubkey>
-        ensures |seqKeysInValidators(xv)| == |xv|
-        decreases xv
+    predicate isValidProposerSlashings(s: BeaconState, bb: BeaconBlockBody)
+        requires minimumActiveValidators(s)
+        requires  |s.validators| == |s.balances|
     {
-        if |xv| == 0 then  
-            []
-        else 
-            [ xv[0].pubkey ] + seqKeysInValidators(xv[1..])
+        // proposer slashing preconditions
+        (forall i,j :: 0 <= i < j < |bb.proposer_slashings| && i != j ==> bb.proposer_slashings[i].header_1.proposer_index!= bb.proposer_slashings[j].header_1.proposer_index) // ve indices are unique
+        &&
+        (forall i :: 0 <= i < |bb.proposer_slashings| ==> 
+            bb.proposer_slashings[i].header_1.slot == bb.proposer_slashings[i].header_2.slot
+            && bb.proposer_slashings[i].header_1.proposer_index == bb.proposer_slashings[i].header_2.proposer_index
+            && bb.proposer_slashings[i].header_1 == bb.proposer_slashings[i].header_2
+            && bb.proposer_slashings[i].header_1.proposer_index as int < |s.validators| 
+            && !s.validators[bb.proposer_slashings[i].header_1.proposer_index].slashed 
+            && s.validators[bb.proposer_slashings[i].header_1.proposer_index].activation_epoch <= get_current_epoch(s) < s.validators[bb.proposer_slashings[i].header_1.proposer_index].withdrawable_epoch)
     }
 
-    /**
-     *  Collect pubkey in a list of deposits.
-     *
-     *  @param  xd  A list of validators,
-     *  @returns    The sequence\list of keys held by the depositors in `xd`.
-     */
-    function method seqKeysInDeposits(xd : seq<Deposit>) : seq<BLSPubkey>
-        ensures |seqKeysInDeposits(xd)| == |xd|
-        decreases xd
+    predicate isValidAttesterSlashings(s: BeaconState, bb: BeaconBlockBody)
+        requires minimumActiveValidators(s)
+        requires  |s.validators| == |s.balances|
     {
-        if |xd| == 0 then  
-            []
-        else 
-            [ xd[0].data.pubkey ] + seqKeysInDeposits(xd[1..])
+        // attester slashing preconditions
+        (forall i :: 0 <= i < |bb.attester_slashings| ==> 
+            forall j :: 0 <= j < |bb.attester_slashings[i].attestation_1.attesting_indices| ==> bb.attester_slashings[i].attestation_1.attesting_indices[j] as int < |s.validators| )
+
+        && (forall i :: 0 <= i < |bb.attester_slashings| ==> 
+            forall j :: 0 <= j < |bb.attester_slashings[i].attestation_2.attesting_indices| ==> bb.attester_slashings[i].attestation_2.attesting_indices[j] as int < |s.validators|)
+            
+        && (forall i :: 0 <= i < |bb.attester_slashings| ==> 
+            && is_valid_indexed_attestation(s, bb.attester_slashings[i].attestation_1)
+            && is_valid_indexed_attestation(s, bb.attester_slashings[i].attestation_2)
+            && |sorted_intersection(bb.attester_slashings[i].attestation_1.attesting_indices, bb.attester_slashings[i].attestation_2.attesting_indices)| > 0
+            && is_slashable_attestation_data(bb.attester_slashings[i].attestation_1.data, bb.attester_slashings[i].attestation_2.data)
+            && is_valid_indexed_attestation(s, bb.attester_slashings[i].attestation_1)
+            && is_valid_indexed_attestation(s, bb.attester_slashings[i].attestation_2)
+            && |sorted_intersection(bb.attester_slashings[i].attestation_1.attesting_indices, bb.attester_slashings[i].attestation_2.attesting_indices)| > 0
+        )
     }
 
-    
-   
-
-
-    function total_deposits(deposits: seq<Deposit>): nat
+    predicate isValidAttestations(s: BeaconState, bb: BeaconBlockBody)
+        requires minimumActiveValidators(s)
+        requires  |s.validators| == |s.balances|
     {
-        if |deposits| == 0 then 0
-        //else deposits[0].data.amount as nat + total_deposits(deposits[1..])
-        else total_deposits(deposits[..|deposits|-1]) + deposits[|deposits|-1].data.amount as nat
+        // process attestation preconditions
+        |bb.attestations| as nat <= MAX_ATTESTATIONS as nat
+        && (forall i:: 0 <= i < |bb.attestations| ==> attestationIsWellFormed(s, bb.attestations[i]))
+        && |s.current_epoch_attestations| as nat + |bb.attestations| as nat <= MAX_ATTESTATIONS as nat * SLOTS_PER_EPOCH as nat 
+        && |s.previous_epoch_attestations| as nat + |bb.attestations| as nat <= MAX_ATTESTATIONS as nat * SLOTS_PER_EPOCH as nat 
     }
 
-    function total_balances(bal: seq<Gwei>): nat
+    predicate isValidDeposits(s: BeaconState, bb: BeaconBlockBody)
+        requires minimumActiveValidators(s)
+        requires  |s.validators| == |s.balances|
     {
-        if |bal| == 0 then 0
-        else bal[0] as nat + total_balances(bal[1..])
+        // process deposit preconditions
+        (s.eth1_deposit_index as int +  |bb.deposits| < 0x10000000000000000 )
+        && (|s.validators| + |bb.deposits| <= VALIDATOR_REGISTRY_LIMIT as int)
+        && (total_balances(s.balances) + total_deposits(bb.deposits) < 0x10000000000000000 )
     }
 
-        /**
-     * Extract a validator from a single deposit.
-     *
-     *  @param  d       A single deposit.
-     *  @returns        A validator created from the deposit information
-     *
-     *  @note           The `effective_balance` is not an active field in the current model but the code
-     *                  to set this field is included as a comment for future reference.
-     */
-    function method get_validator_from_deposit(d: Deposit): Validator
-        ensures get_validator_from_deposit(d).effective_balance <= MAX_EFFECTIVE_BALANCE as Gwei
+    predicate isValidVoluntaryExits(s: BeaconState, bb: BeaconBlockBody)
+        requires minimumActiveValidators(s)
+        requires  |s.validators| == |s.balances|
     {
-        var amount := d.data.amount; 
-        var effective_balance := min((amount as nat- amount as nat % EFFECTIVE_BALANCE_INCREMENT as nat) as nat, MAX_EFFECTIVE_BALANCE as nat);
-
-        Validator(d.data.pubkey, effective_balance as Gwei, false, FAR_FUTURE_EPOCH, FAR_FUTURE_EPOCH, FAR_FUTURE_EPOCH, FAR_FUTURE_EPOCH)
+        // voluntary exit preconditions
+        (forall i,j :: 0 <= i < j < |bb.voluntary_exits| && i != j ==> bb.voluntary_exits[i].validator_index != bb.voluntary_exits[j].validator_index )// ve indices are unique
+        && (forall i :: 0 <= i < |bb.voluntary_exits| ==> 
+             bb.voluntary_exits[i].validator_index as int < |s.validators| 
+             && get_current_epoch(s) >= bb.voluntary_exits[i].epoch
+             && !s.validators[bb.voluntary_exits[i].validator_index].slashed
+             && s.validators[bb.voluntary_exits[i].validator_index].activation_epoch <= get_current_epoch(s) < s.validators[bb.voluntary_exits[i].validator_index].withdrawable_epoch
+             && s.validators[bb.voluntary_exits[i].validator_index].exitEpoch == FAR_FUTURE_EPOCH
+             && (get_current_epoch(s) as nat >= s.validators[bb.voluntary_exits[i].validator_index].activation_epoch as nat + SHARD_COMMITTEE_PERIOD as nat)
+            )
     }
 
-    /**
-     *  Append a new validator
-     */
-    function method validator_append(sv: ListOfValidators, v: Validator): ListOfValidators
-        requires |sv| + 1 <= VALIDATOR_REGISTRY_LIMIT as int
+    predicate isValidBeaconBlockBody(s: BeaconState, bb: BeaconBlockBody)
+        requires minimumActiveValidators(s)
+        requires  |s.validators| == |s.balances|
+        // Note: A proof could be constructed to show that the intermediate states apply for s as well.
+        //      i.e. try to show the preconditions based on state s
     {
-        sv + [v]
-    }
-    /**
-     *  Append a new balance entry
-     */
-    function method balance_append(sb: ListOfBalances, b: Gwei): ListOfBalances
-        requires |sb| + 1 <= VALIDATOR_REGISTRY_LIMIT as int
-    {
-        sb + [b]
+        isValidProposerSlashings(s, bb)
+        && isValidAttesterSlashings(updateProposerSlashings(s, bb.proposer_slashings), bb)
+        && isValidAttestations(updateAttesterSlashings(updateProposerSlashings(s, bb.proposer_slashings), bb.attester_slashings), bb)
+        && isValidDeposits(updateAttestations(updateAttesterSlashings(updateProposerSlashings(s, bb.proposer_slashings), bb.attester_slashings), bb.attestations),bb)
+        && isValidVoluntaryExits(updateDeposits(updateAttestations(updateAttesterSlashings(updateProposerSlashings(s, bb.proposer_slashings), bb.attester_slashings), bb.attestations),bb.deposits),bb)
     }
 
-     /**
-     *  Get the index of a validator. 
-     *
-     *  @notes  Helper function as no alternative indexing functionality available.
-     *
-     */
-    function method get_validator_index(pk: seq<BLSPubkey>, pubkey: BLSPubkey) : ValidatorIndex
-        requires |pk| < VALIDATOR_REGISTRY_LIMIT as int
-        requires pubkey in pk
-        ensures get_validator_index(pk,pubkey) as int < |pk|
-        ensures pk[get_validator_index(pk,pubkey)] == pubkey
-        decreases pk
-    {
-        if pk[0] == pubkey then 0 as ValidatorIndex
-        else 1 + get_validator_index(pk[1..], pubkey)
-        // alternative reverse form
-        //if pk[|pk|-1] == pubkey then (|pk|-1) as ValidatorIndex
-        //else get_validator_index(pk[..|pk|-1], pubkey)
+    function updateOperations(s: BeaconState, bb: BeaconBlockBody): BeaconState
+        requires  |s.validators| == |s.balances|
+        requires |get_active_validator_indices(s.validators, get_current_epoch(s))| > 0
+        requires isValidBeaconBlockBody(s, bb)
 
+        ensures updateOperations(s, bb) == updateVoluntaryExits(updateDeposits(updateAttestations(updateAttesterSlashings(updateProposerSlashings(s, bb.proposer_slashings), bb.attester_slashings), bb.attestations), bb.deposits), bb.voluntary_exits)
+    {
+        //assert isValidProposerSlashings(s, bb);
+        var s1 := updateProposerSlashings(s, bb.proposer_slashings);
+        assert s1 == updateProposerSlashings(s, bb.proposer_slashings);
+        //assert get_current_epoch(s1) == get_current_epoch(s);
+        
+        var s2 := updateAttesterSlashings(s1, bb.attester_slashings);
+        assert s2 == updateAttesterSlashings(updateProposerSlashings(s, bb.proposer_slashings), bb.attester_slashings);
+        
+        var s3 := updateAttestations(s2, bb.attestations);
+        assert s3 == updateAttestations(updateAttesterSlashings(updateProposerSlashings(s, bb.proposer_slashings), bb.attester_slashings), bb.attestations);
+        
+        var s4 := updateDeposits(s3, bb.deposits);
+        assert s4 == updateDeposits(updateAttestations(updateAttesterSlashings(updateProposerSlashings(s, bb.proposer_slashings), bb.attester_slashings), bb.attestations), bb.deposits);
+
+         var s5 := updateVoluntaryExits(s4, bb.voluntary_exits);
+        assert s5 == updateVoluntaryExits(updateDeposits(updateAttestations(updateAttesterSlashings(updateProposerSlashings(s, bb.proposer_slashings), bb.attester_slashings), bb.attestations), bb.deposits), bb.voluntary_exits);
+        
+        s5
     }
 
     
@@ -252,112 +262,9 @@ module ProcessOperationsSpec {
         )
     }
 
-    // function total_deposits(deposits: seq<Deposit>): nat
-    // {
-    //     if |deposits| == 0 then 0
-    //     //else deposits[0].data.amount as nat + total_deposits(deposits[1..])
-    //     else total_deposits(deposits[..|deposits|-1]) + deposits[|deposits|-1].data.amount as nat
-    // }
 
-    // function total_balances(bal: seq<Gwei>): nat
-    // {
-    //     if |bal| == 0 then 0
-    //     else bal[0] as nat + total_balances(bal[1..])
-    // }
 
-        /**
-     * Extract a validator from a single deposit.
-     *
-     *  @param  d       A single deposit.
-     *  @returns        A validator created from the deposit information
-     *
-     *  @note           The `effective_balance` is not an active field in the current model but the code
-     *                  to set this field is included as a comment for future reference.
-     */
-    // function method get_validator_from_deposit(d: Deposit): Validator
-    //     ensures get_validator_from_deposit(d).effective_balance <= MAX_EFFECTIVE_BALANCE as Gwei
-    // {
-    //     var amount := d.data.amount; 
-    //     var effective_balance := min((amount as int- amount as int % EFFECTIVE_BALANCE_INCREMENT) as nat, MAX_EFFECTIVE_BALANCE as nat);
-
-    //     Validator(d.data.pubkey, effective_balance as Gwei)
-    // }
-
-    /**
-     *  Append a new validator
-     */
-    // function method validator_append(sv: ListOfValidators, v: Validator): ListOfValidators
-    //     requires |sv| + 1 <= VALIDATOR_REGISTRY_LIMIT as int
-    // {
-    //     sv + [v]
-    // }
-    /**
-     *  Append a new balance entry
-     */
-    // function method balance_append(sb: ListOfBalances, b: Gwei): ListOfBalances
-    //     requires |sb| + 1 <= VALIDATOR_REGISTRY_LIMIT as int
-    // {
-    //     sb + [b]
-    // }
-
-     /**
-     *  Get the index of a validator. 
-     *
-     *  @notes  Helper function as no alternative indexing functionality available.
-     *
-     */
-    // function method get_validator_index(pk: seq<BLSPubkey>, pubkey: BLSPubkey) : ValidatorIndex
-    //     requires |pk| < VALIDATOR_REGISTRY_LIMIT as int
-    //     requires pubkey in pk
-    //     ensures get_validator_index(pk,pubkey) as int < |pk|
-    //     ensures pk[get_validator_index(pk,pubkey)] == pubkey
-    //     decreases pk
-    // {
-    //     if pk[0] == pubkey then 0 as ValidatorIndex
-    //     else 1 + get_validator_index(pk[1..], pubkey)
-    //     // alternative reverse form
-    //     //if pk[|pk|-1] == pubkey then (|pk|-1) as ValidatorIndex
-    //     //else get_validator_index(pk[..|pk|-1], pubkey)
-
-    // }
-
-    // Beacon State Mutators
-
-    /** increase_balance
-     *  Increase the validator balance at index ``index`` by ``delta``.
-     *  
-     **/
-    function method increase_balance(s: BeaconState, index: ValidatorIndex, delta: Gwei): BeaconState 
-        requires index as int < |s.balances| 
-        requires s.balances[index] as int + delta as int < 0x10000000000000000
-        ensures |s.balances| == |increase_balance(s,index,delta).balances|
-        ensures increase_balance(s,index,delta).balances[index] == s.balances[index] + delta
-    {
-        s.(
-            balances := s.balances[index as int := (s.balances[index] + delta)]
-        )
-    }
-
-    /** decrease_balance
-     *  Decrease the validator balance at index ``index`` by ``delta``.
-     *
-     **/
-    function method decrease_balance(s: BeaconState, index: ValidatorIndex, delta: Gwei): BeaconState 
-        requires index as int < |s.balances| 
-        ensures |s.balances| == |decrease_balance(s,index,delta).balances|
-        ensures if s.balances[index] > delta then decrease_balance(s,index,delta).balances[index] == s.balances[index] - delta
-                else decrease_balance(s,index,delta).balances[index] == 0
-        ensures s.validators == decrease_balance(s,index,delta).validators
-    {
-        if s.balances[index] > delta then
-            s.(
-                balances := s.balances[index as int := (s.balances[index] - delta)]
-            )
-        else
-            s.(
-                balances := s.balances[index as int := 0]
-            )
-    }
+    
 
     ///////////////////////
     predicate attestationIsWellFormed(s: BeaconState, a: Attestation)
@@ -500,23 +407,6 @@ module ProcessOperationsSpec {
             updateAttestation(s1, a[index])
     }
 
-    lemma AttestationHelperLemma(s: BeaconState, s1: BeaconState, a: Attestation)
-        requires attestationIsWellFormed(s, a);
-        requires s1.validators == s.validators
-        requires s1.slot == s.slot
-        requires s1.current_justified_checkpoint == s.current_justified_checkpoint
-        requires s1.previous_justified_checkpoint == s.previous_justified_checkpoint
-        ensures attestationIsWellFormed(s1, a);
-    {
-        
-    }
-
-        
-
-
-
-
-
     function updateVoluntaryExit(s: BeaconState, voluntary_exit: VoluntaryExit) : BeaconState
         requires |s.validators| == |s.balances|
         requires voluntary_exit.validator_index as int < |s.validators| 
@@ -579,55 +469,7 @@ module ProcessOperationsSpec {
 
     }
 
-    lemma VolExitLemma1(s: BeaconState, voluntary_exit: VoluntaryExit)
-        requires |s.validators| == |s.balances|
-        requires voluntary_exit.validator_index as int < |s.validators| 
-        requires minimumActiveValidators(s)
-        
-        requires !s.validators[voluntary_exit.validator_index].slashed
-        requires s.validators[voluntary_exit.validator_index].activation_epoch <= get_current_epoch(s) < s.validators[voluntary_exit.validator_index].withdrawable_epoch
-
-        requires s.validators[voluntary_exit.validator_index].exitEpoch == FAR_FUTURE_EPOCH
-        requires get_current_epoch(s) >= voluntary_exit.epoch
-        requires get_current_epoch(s) >= s.validators[voluntary_exit.validator_index].activation_epoch + SHARD_COMMITTEE_PERIOD 
-
-        ensures minimumActiveValidators(updateVoluntaryExit(s, voluntary_exit))
-    {
-        // var s1 := updateVoluntaryExit(s, voluntary_exit);
-        // assert get_current_epoch(s) == get_current_epoch(s1);
-        // assert exists v :: 0 <= v < |s.validators| && s.validators[v].activation_epoch <= get_current_epoch(s) < s.validators[v].exitEpoch;
-        // assert forall v :: 0 <= v < |s.validators| ==> s.validators[v].activation_epoch <= get_current_epoch(s) < s.validators[v].exitEpoch
-        //                                             ==> s1.validators[v].activation_epoch <= get_current_epoch(s1) < s1.validators[v].exitEpoch;
-        // assert exists v :: 0 <= v < |s1.validators| && s1.validators[v].activation_epoch <= get_current_epoch(s1) < s1.validators[v].exitEpoch;
-        // assert exists v :: 0 <= v < |s1.validators| && is_active_validator(s1.validators[v], get_current_epoch(s1));
-        // assert |get_active_validator_indices(s1.validators, get_current_epoch(s1))| > 0 ==> 
-        //     (exists v :: 0 <= v < |s1.validators| && is_active_validator(s1.validators[v], get_current_epoch(s1)));
-        // assert  minimumActiveValidators(s1);
-    }
-
     
-
-    lemma helperVoluntaryExitLemma3(s: BeaconState, ve: seq<VoluntaryExit>)
-        requires forall i :: 0 <= i < |ve| ==> ve[i].validator_index as int < |s.validators| 
-        //requires forall i :: 0 <= i < |ve| ==> is_active_validator(s.validators[ve[i].validator_index], get_current_epoch(s))
-        requires forall i :: 0 <= i < |ve| ==> !s.validators[ve[i].validator_index].slashed
-        requires forall i :: 0 <= i < |ve| ==> s.validators[ve[i].validator_index].activation_epoch <= get_current_epoch(s) < s.validators[ve[i].validator_index].withdrawable_epoch
-
-        requires forall i :: 0 <= i < |ve| ==> s.validators[ve[i].validator_index].exitEpoch == FAR_FUTURE_EPOCH
-        requires forall i :: 0 <= i < |ve| ==> get_current_epoch(s) >= s.validators[ve[i].validator_index].activation_epoch + SHARD_COMMITTEE_PERIOD 
-
-        ensures forall i :: i in get_VolExit_validator_indices(ve) ==> 0 <= i < |s.validators| 
-        
-        //ensures forall i :: i in get_VolExit_validator_indices(ve) ==> is_active_validator(s.validators[i], get_current_epoch(s))
-        ensures forall i :: i in get_VolExit_validator_indices(ve) ==> !s.validators[i].slashed
-        ensures forall i :: i in get_VolExit_validator_indices(ve) ==> s.validators[i].activation_epoch <= get_current_epoch(s) < s.validators[i].withdrawable_epoch
-
-        ensures forall i :: i in get_VolExit_validator_indices(ve) ==> s.validators[i].exitEpoch == FAR_FUTURE_EPOCH
-        ensures forall i :: i in get_VolExit_validator_indices(ve) ==> get_current_epoch(s) >= s.validators[i].activation_epoch + SHARD_COMMITTEE_PERIOD 
-    {
-        // Thanks Dafny
-    }
-
     
     function {:timeLimitMultiplier 1} updateVoluntaryExits(s: BeaconState, ve: seq<VoluntaryExit>) : BeaconState
         requires minimumActiveValidators(s)
@@ -716,193 +558,11 @@ module ProcessOperationsSpec {
             updateVoluntaryExit(updateVoluntaryExits(s,ve[..|ve|-1]), ve[|ve|-1])
     }
 
-    lemma helperVoluntaryExitLemma2(s: BeaconState, ve: seq<VoluntaryExit>)
-        requires  |get_VolExit_validator_indices(ve)| > 0
-        requires forall i :: i in get_VolExit_validator_indices(ve) ==> 0 <= i < |s.validators| 
-        requires forall i :: i in get_VolExit_validator_indices(ve) ==> !s.validators[i].slashed
-        requires forall i :: i in get_VolExit_validator_indices(ve) ==> s.validators[i].activation_epoch <= get_current_epoch(s) < s.validators[i].withdrawable_epoch
-        requires forall i :: i in get_VolExit_validator_indices(ve) ==> s.validators[i].exitEpoch == FAR_FUTURE_EPOCH
-        requires forall i :: i in get_VolExit_validator_indices(ve) ==> get_current_epoch(s) >= s.validators[i].activation_epoch + SHARD_COMMITTEE_PERIOD 
     
-
-        ensures forall i :: i in get_VolExit_validator_indices(ve[..|ve|-1]) ==> 0 <= i < |s.validators|
-        ensures forall i :: i in get_VolExit_validator_indices(ve[..|ve|-1]) ==> !s.validators[i].slashed
-        ensures forall i :: i in get_VolExit_validator_indices(ve[..|ve|-1]) ==> s.validators[i].activation_epoch <= get_current_epoch(s) < s.validators[i].withdrawable_epoch
-        ensures forall i :: i in get_VolExit_validator_indices(ve[..|ve|-1]) ==> s.validators[i].exitEpoch == FAR_FUTURE_EPOCH
-        ensures forall i :: i in get_VolExit_validator_indices(ve[..|ve|-1]) ==> get_current_epoch(s) >= s.validators[i].activation_epoch + SHARD_COMMITTEE_PERIOD
-    {
-        mappingVolExitIndices(ve);
-        assert forall i :: 0 <= i < |ve| ==> get_VolExit_validator_indices(ve)[i] == ve[i].validator_index as int;
-
-        subsetMappingVolExitIndices(ve, |ve|-1);
-        assert get_VolExit_validator_indices(ve[..|ve|-1]) == get_VolExit_validator_indices(ve)[..|ve|-1];
-        
-        assert forall i :: i in get_VolExit_validator_indices(ve) ==> 0 <= i < |s.validators|; // from requires
-        assert forall i :: 0 <= i < |ve| ==> get_VolExit_validator_indices(ve)[i] == ve[i].validator_index as int;
-        assert forall i :: 0 <= i < |ve| ==> ve[i].validator_index as int in get_VolExit_validator_indices(ve) ;
-        
-    }
-
-    lemma helperVoluntaryExitLemma(s: BeaconState, exit: VoluntaryExit)
-        requires |s.validators| == |s.balances|
-        requires exit.validator_index as int < |s.validators| 
-        // requires is_active_validator(s.validators[voluntary_exit.validator_index], get_current_epoch(s))
-        // (!v.slashed) && (v.activation_epoch <= epoch < v.withdrawable_epoch)
-        requires !s.validators[exit.validator_index].slashed
-        requires s.validators[exit.validator_index].activation_epoch <= get_current_epoch(s) < s.validators[exit.validator_index].withdrawable_epoch
-
-        requires s.validators[exit.validator_index].exitEpoch == FAR_FUTURE_EPOCH
-        requires get_current_epoch(s) >= exit.epoch
-        requires get_current_epoch(s) >= s.validators[exit.validator_index].activation_epoch + SHARD_COMMITTEE_PERIOD 
-        
-        ensures forall i :: 0 <= i < |s.validators| && i != exit.validator_index as int ==> updateVoluntaryExit(s, exit).validators[i].exitEpoch == s.validators[i].exitEpoch
-        ensures forall i :: 0 <= i < |s.validators| && i != exit.validator_index as int ==> updateVoluntaryExit(s, exit).validators[i].slashed == s.validators[i].slashed
-        ensures forall i :: 0 <= i < |s.validators| && i != exit.validator_index as int ==> updateVoluntaryExit(s, exit).validators[i].withdrawable_epoch == s.validators[i].withdrawable_epoch
-    {
-        // Thanks Dafny
-    }
-
- 
-    function get_VolExit_validator_indices(ve: seq<VoluntaryExit>): seq<int>
-        ensures |get_VolExit_validator_indices(ve)| == |ve|
-    {
-        if |ve| == 0 then []
-        else [ve[0].validator_index as int] + get_VolExit_validator_indices(ve[1..])
-    }
-
-    lemma mappingVolExitIndices(ve: seq<VoluntaryExit>)
-        ensures forall i :: 0 <= i < |ve| ==> get_VolExit_validator_indices(ve)[i] == ve[i].validator_index as int
-    {
-        //Thanks Dafny
-    }
-
-    lemma subsetMappingVolExitIndices(ve: seq<VoluntaryExit>, i : nat)
-        requires 0 <= i < |ve|
-        ensures get_VolExit_validator_indices(ve[..i]) == get_VolExit_validator_indices(ve)[..i]
-    {
-        if |ve| == 0 {}
-        else {
-            assert ve == ve[..i] + ve[i..];
-            
-            mappingVolExitIndices(ve[..i]);
-            assert forall j :: 0 <= j < |ve[..i]| ==> get_VolExit_validator_indices(ve[..i])[j] == ve[j].validator_index as int;
-
-            mappingVolExitIndices(ve);
-            assert forall j :: 0 <= j < |ve| ==> get_VolExit_validator_indices(ve)[j] == ve[j].validator_index as int;
-        }
-    }
-
-    //lemma PSpreconditionLemma()
-    lemma helperVolExitLemma4(ve : seq<VoluntaryExit>)
-        requires |ve| > 0
-        requires forall i,j :: 0 <= i < j < |ve| && i != j ==> ve[i].validator_index!= ve[j].validator_index // ve indices are unique
-        ensures ve[|ve|-1].validator_index as int !in get_VolExit_validator_indices(ve[..|ve|-1])
-    {
-        mappingVolExitIndices(ve[..|ve|-1]);
-        assert forall i :: 0 <= i < |ve[..|ve|-1]| ==> get_VolExit_validator_indices(ve[..|ve|-1])[i] == ve[i].validator_index as int;
-    }
-
-///////////////////////////
-
-    function get_PS_validator_indices(ps: seq<ProposerSlashing>): seq<int>
-        ensures |get_PS_validator_indices(ps)| == |ps|
-    {
-        if |ps| == 0 then []
-        else [ps[0].header_1.proposer_index as int] + get_PS_validator_indices(ps[1..])
-    }
-
-    lemma mappingPSIndices(ps: seq<ProposerSlashing>)
-        ensures forall i :: 0 <= i < |ps| ==> get_PS_validator_indices(ps)[i] == ps[i].header_1.proposer_index as int
-    {
-        //Thanks Dafny
-    }
-
-    lemma subsetMappingPSIndices(ps: seq<ProposerSlashing>, i : nat)
-        requires 0 <= i < |ps|
-        ensures get_PS_validator_indices(ps[..i]) == get_PS_validator_indices(ps)[..i]
-    {
-        if |ps| == 0 {}
-        else {
-            assert ps == ps[..i] + ps[i..];
-            
-            mappingPSIndices(ps[..i]);
-            assert forall j :: 0 <= j < |ps[..i]| ==> get_PS_validator_indices(ps[..i])[j] == ps[j].header_1.proposer_index as int;
-
-            mappingPSIndices(ps);
-            assert forall j :: 0 <= j < |ps| ==> get_PS_validator_indices(ps)[j] == ps[j].header_1.proposer_index as int;
-        }
-    }
-
-    lemma helperPSLemma(s: BeaconState, ps: ProposerSlashing)
-        requires ps.header_1.slot == ps.header_2.slot
-        requires ps.header_1.proposer_index == ps.header_2.proposer_index 
-        requires ps.header_1 == ps.header_2
-        requires ps.header_1.proposer_index as int < |s.validators| 
-
-        // requires is_active_validator: (!v.slashed) && (v.activation_epoch <= epoch < v.withdrawable_epoch)
-        requires !s.validators[ps.header_1.proposer_index].slashed
-        requires s.validators[ps.header_1.proposer_index].activation_epoch <= get_current_epoch(s) < s.validators[ps.header_1.proposer_index].withdrawable_epoch
- 
-        requires |get_active_validator_indices(s.validators, get_current_epoch(s))| > 0
-        requires |s.validators| == |s.balances|
-        
-        ensures forall i :: 0 <= i < |s.validators| && i != ps.header_1.proposer_index as int ==> updateProposerSlashing(s, ps).validators[i].exitEpoch == s.validators[i].exitEpoch
-        ensures forall i :: 0 <= i < |s.validators| && i != ps.header_1.proposer_index as int ==> updateProposerSlashing(s, ps).validators[i].slashed == s.validators[i].slashed
-        ensures forall i :: 0 <= i < |s.validators| && i != ps.header_1.proposer_index as int ==> updateProposerSlashing(s, ps).validators[i].withdrawable_epoch == s.validators[i].withdrawable_epoch
-    {
-        // Thanks Dafny
-    }
-
-    lemma helperPSLemma2(s: BeaconState, ps: seq<ProposerSlashing>)
-        requires  |get_PS_validator_indices(ps)| > 0
-        requires forall i :: i in get_PS_validator_indices(ps) ==> 0 <= i < |s.validators| 
-        requires forall i :: i in get_PS_validator_indices(ps) ==> !s.validators[i].slashed
-        requires forall i :: i in get_PS_validator_indices(ps) ==> s.validators[i].activation_epoch <= get_current_epoch(s) < s.validators[i].withdrawable_epoch
-        
-
-        ensures forall i :: i in get_PS_validator_indices(ps[..|ps|-1]) ==> 0 <= i < |s.validators|
-        ensures forall i :: i in get_PS_validator_indices(ps[..|ps|-1]) ==> !s.validators[i].slashed
-        ensures forall i :: i in get_PS_validator_indices(ps[..|ps|-1]) ==> s.validators[i].activation_epoch <= get_current_epoch(s) < s.validators[i].withdrawable_epoch
-    {
-        mappingPSIndices(ps);
-        assert forall i :: 0 <= i < |ps| ==> get_PS_validator_indices(ps)[i] == ps[i].header_1.proposer_index as int;
-
-        subsetMappingPSIndices(ps, |ps|-1);
-        assert get_PS_validator_indices(ps[..|ps|-1]) == get_PS_validator_indices(ps)[..|ps|-1];
-        
-        assert forall i :: i in get_PS_validator_indices(ps) ==> 0 <= i < |s.validators|; // from requires
-        assert forall i :: 0 <= i < |ps| ==> get_PS_validator_indices(ps)[i] == ps[i].header_1.proposer_index as int;
-        assert forall i :: 0 <= i < |ps| ==> ps[i].header_1.proposer_index as int in get_PS_validator_indices(ps) ;
-        
-    }
-
+    
 
     
 
-    lemma updateProposerSlashingLemma(s: BeaconState, ps : ProposerSlashing)
-        requires ps.header_1.slot == ps.header_2.slot
-        requires ps.header_1.proposer_index == ps.header_2.proposer_index 
-        requires ps.header_1 == ps.header_2
-        requires ps.header_1.proposer_index as int < |s.validators| 
-        //requires is_slashable_validator(s.validators[ps.header_1.proposer_index], get_current_epoch(s));
-        //(!v.slashed) && (v.activation_epoch <= epoch < v.withdrawable_epoch)
-        requires !s.validators[ps.header_1.proposer_index].slashed
-        requires s.validators[ps.header_1.proposer_index].activation_epoch <= get_current_epoch(s) < s.validators[ps.header_1.proposer_index].withdrawable_epoch
-        
-        requires |get_active_validator_indices(s.validators, get_current_epoch(s))| > 0
-        requires |s.validators| == |s.balances|
-        
-        ensures |get_active_validator_indices(updateProposerSlashing(s, ps).validators, get_current_epoch(s))| > 0
-    {
-        var index := ps.header_1.proposer_index; // validator to be slashed
-        var slashable_validator := s.validators[index];
-        var epoch : Epoch := get_current_epoch(s);
-
-        assert updateProposerSlashing(s, ps) == slash_validator(s, ps.header_1.proposer_index, get_beacon_proposer_index(s));
-        slashValidatorPreservesActivateValidators(s, ps.header_1.proposer_index, get_beacon_proposer_index(s));
-        assert |get_active_validator_indices(updateProposerSlashing(s, ps).validators, get_current_epoch(s))| > 0;
-
-    }
 
 
     function updateProposerSlashing(s: BeaconState, ps : ProposerSlashing) : BeaconState 
@@ -940,58 +600,7 @@ module ProcessOperationsSpec {
         // maybe expand???
     }
 
-    lemma helperPSLemma3(s: BeaconState, ps : seq<ProposerSlashing>)
-        requires forall i :: 0 <= i < |ps| ==> ps[i].header_1.proposer_index as int < |s.validators| 
-        requires forall i :: 0 <= i < |ps| ==> !s.validators[ps[i].header_1.proposer_index].slashed 
-        requires forall i :: 0 <= i < |ps| ==> s.validators[ps[i].header_1.proposer_index].activation_epoch <= get_current_epoch(s) < s.validators[ps[i].header_1.proposer_index].withdrawable_epoch
-
-        ensures forall i :: i in get_PS_validator_indices(ps) ==> 0 <= i < |s.validators|
-        ensures forall i :: i in get_PS_validator_indices(ps) ==> !s.validators[i].slashed
-        ensures forall i :: i in get_PS_validator_indices(ps) ==> s.validators[i].activation_epoch <= get_current_epoch(s) < s.validators[i].withdrawable_epoch
-    {
-        // Thanks Dafny
-    }
-
-    lemma helperPSLemma4(ps : seq<ProposerSlashing>)
-        requires |ps| > 0
-        requires forall i,j :: 0 <= i < j < |ps| && i != j ==> ps[i].header_1.proposer_index!= ps[j].header_1.proposer_index // ve indices are unique
-        ensures ps[|ps|-1].header_1.proposer_index as int !in get_PS_validator_indices(ps[..|ps|-1])
-    {
-        mappingPSIndices(ps[..|ps|-1]);
-        assert forall i :: 0 <= i < |ps[..|ps|-1]| ==> get_PS_validator_indices(ps[..|ps|-1])[i] == ps[i].header_1.proposer_index as int;
-    }
-
-    lemma helperPSLemma5(s: BeaconState, ps : seq<ProposerSlashing>)
-        requires |ps| > 0
-        requires forall i,j :: 0 <= i < j < |ps| && i != j ==> ps[i].header_1.proposer_index!= ps[j].header_1.proposer_index // ve indices are unique
-        requires forall i :: 0 <= i < |ps| ==> ps[i].header_1.slot == ps[i].header_2.slot
-        requires forall i :: 0 <= i < |ps| ==> ps[i].header_1.proposer_index == ps[i].header_2.proposer_index 
-        requires forall i :: 0 <= i < |ps| ==> ps[i].header_1 == ps[i].header_2
-        requires forall i :: 0 <= i < |ps| ==> ps[i].header_1.proposer_index as int < |s.validators| 
-        requires forall i :: 0 <= i < |ps| ==> !s.validators[ps[i].header_1.proposer_index].slashed 
-        requires forall i :: 0 <= i < |ps| ==> s.validators[ps[i].header_1.proposer_index].activation_epoch <= get_current_epoch(s) < s.validators[ps[i].header_1.proposer_index].withdrawable_epoch
-
-        ensures forall i,j :: 0 <= i < j < |ps[..|ps|-1]| && i != j ==> ps[i].header_1.proposer_index!= ps[j].header_1.proposer_index
-        ensures forall i :: 0 <= i < |ps[..|ps|-1]| ==> ps[i].header_1.slot == ps[i].header_2.slot;
-        ensures forall i :: 0 <= i < |ps[..|ps|-1]| ==> ps[i].header_1.proposer_index == ps[i].header_2.proposer_index ;
-        ensures forall i :: 0 <= i < |ps[..|ps|-1]| ==> ps[i].header_1 == ps[i].header_2;
-        ensures forall i :: 0 <= i < |ps[..|ps|-1]| ==> ps[i].header_1.proposer_index as int < |s.validators| ;
-        ensures forall i :: 0 <= i < |ps[..|ps|-1]| ==> !s.validators[ps[i].header_1.proposer_index].slashed ;
-        ensures forall i :: 0 <= i < |ps[..|ps|-1]| ==> s.validators[ps[i].header_1.proposer_index].activation_epoch <= get_current_epoch(s) < s.validators[ps[i].header_1.proposer_index].withdrawable_epoch;
-           
-    {
-    }
-
-    lemma helperPSLemma6(ps : seq<ProposerSlashing>)
-        requires |ps| > 0
-        ensures get_PS_validator_indices(ps[..|ps|-1]) + [ps[|ps|-1].header_1.proposer_index as int] == get_PS_validator_indices(ps)
-        ensures forall i : int :: i !in get_PS_validator_indices(ps[..|ps|-1]) && i != ps[|ps|-1].header_1.proposer_index as int ==>
-                i !in get_PS_validator_indices(ps)
-    {
-        mappingPSIndices(ps);
-        subsetMappingPSIndices(ps, |ps|-1);
-    }
-
+    
 
     function updateProposerSlashings(s: BeaconState, ps : seq<ProposerSlashing>) : BeaconState
         requires minimumActiveValidators(s)
@@ -1069,89 +678,8 @@ module ProcessOperationsSpec {
 
     }
 
-    // lemma helperPSLemma7(s: BeaconState, ps : seq<ProposerSlashing>)
-    //     //requires |ps| > 0
-    //     requires forall i,j :: 0 <= i < j < |ps| && i != j ==> ps[i].header_1.proposer_index!= ps[j].header_1.proposer_index // ve indices are unique
-        
-    //     requires forall i :: 0 <= i < |ps| ==> ps[i].header_1.slot == ps[i].header_2.slot
-    //     requires forall i :: 0 <= i < |ps| ==> ps[i].header_1.proposer_index == ps[i].header_2.proposer_index 
-    //     requires forall i :: 0 <= i < |ps| ==> ps[i].header_1 == ps[i].header_2
-    //     requires forall i :: 0 <= i < |ps| ==> ps[i].header_1.proposer_index as int < |s.validators| 
-    //     requires forall i :: 0 <= i < |ps| ==> !s.validators[ps[i].header_1.proposer_index].slashed 
-    //     requires forall i :: 0 <= i < |ps| ==> s.validators[ps[i].header_1.proposer_index].activation_epoch <= get_current_epoch(s) < s.validators[ps[i].header_1.proposer_index].withdrawable_epoch
-
-    //     ensures forall i :: 0 <= i < |s.validators| && i !in get_PS_validator_indices(ps) ==> updateProposerSlashings(s, ps).validators[i] == s.validators[i]
-        
     
     /////////////////////////////////////////////////////////////////////////////////////
-
-
-    // Helper functions: Sorted intersection of two sequences of unique sorted ValidatorIndex
-    // function method indices_intersection(a : seq<ValidatorIndex>, b: seq<ValidatorIndex>): seq<ValidatorIndex>
-    //     requires forall i,j :: 0 <= i < j < |a| ==> a[i] < a[j]
-    //     requires forall i,j :: 0 <= i < j < |b| ==> b[i] < b[j]
-    
-    //     ensures forall i :: 0 <= i < |indices_intersection(a,b)| ==> 
-    //             indices_intersection(a,b)[i] in a && indices_intersection(a,b)[i] in b
-    //     ensures forall i, j :: 0 <= i < j < |indices_intersection(a,b)| ==> 
-    //             indices_intersection(a,b)[i] != indices_intersection(a,b)[j]
-    // {
-    //     if |a| == 0 then []
-    //     else 
-    //         if a[0] in b then 
-    //             [a[0]]
-    //         else [] + indices_intersection(a[1..], b)
-    // }
-
-    function method sorted_intersection(a : seq<ValidatorIndex>, b: seq<ValidatorIndex>): seq<uint64>
-        requires forall i,j :: 0 <= i < j < |a| ==> a[i] < a[j]
-        requires forall i,j :: 0 <= i < j < |b| ==> b[i] < b[j]
-        ensures forall i,j :: 0 <= i < j < |sorted_intersection(a,b)| ==> sorted_intersection(a,b)[i] < sorted_intersection(a,b)[j]
-        ensures forall i :: 0 <= i < |sorted_intersection(a,b)| ==> sorted_intersection(a,b)[i] as ValidatorIndex in a &&
-                                                                    sorted_intersection(a,b)[i] as ValidatorIndex in b
-        ensures sorted_intersection(a,b) == sorted_intersection_fn(a,b)
-    {
-        if |a| == 0 then []
-        else (if a[0] in b then [a[0] as uint64] else []) + sorted_intersection(a[1..], b)
-    }
-
-    lemma helperIndicesLemma(indices: seq<ValidatorIndex>)
-        requires |indices| > 0
-        ensures forall i :: 0 < i < |indices| ==> indices[..i+1] == indices[..i] + [indices[i]]
-    {
-        // Thanks Dafny
-    }
-
-    lemma helperIndicesLemma2(indices: seq<ValidatorIndex>)
-        requires |indices| > 0
-        ensures indices == indices[..|indices|-1] + [indices[|indices|-1]]
-    {
-        // Thanks Dafny
-    }
-
-    lemma helperIndicesLemma3(indices: seq<uint64>, i: nat)
-        requires 0 <= i < |indices|
-        ensures indices[..i+1] == indices[..i] + [indices[i]]
-    {
-        // Thanks Dafny
-    }
-
-    
-
-
-    function sorted_intersection_fn(a : seq<ValidatorIndex>, b: seq<ValidatorIndex>): seq<uint64>
-        requires forall i,j :: 0 <= i < j < |a| ==> a[i] < a[j]
-        requires forall i,j :: 0 <= i < j < |b| ==> b[i] < b[j]
-        ensures forall i,j :: 0 <= i < j < |sorted_intersection_fn(a,b)| ==> sorted_intersection_fn(a,b)[i] < sorted_intersection_fn(a,b)[j]
-        ensures forall i :: 0 <= i < |sorted_intersection_fn(a,b)| ==> sorted_intersection_fn(a,b)[i] as ValidatorIndex in a &&
-                                                                    sorted_intersection_fn(a,b)[i] as ValidatorIndex in b
-    {
-        if |a| == 0 then []
-        else (if a[0] in b then [a[0] as uint64] else []) + sorted_intersection_fn(a[1..], b)
-    }
-
-    //lemma sorted_intersection_bound(s: BeaconState, a : seq<ValidatorIndex>, b: seq<ValidatorIndex>)
-
 
     function updateAttesterSlashings(s: BeaconState, a: seq<AttesterSlashing>) : BeaconState 
         requires forall i :: 0 <= i < |a| ==> is_valid_indexed_attestation(s, a[i].attestation_1)
@@ -1181,40 +709,8 @@ module ProcessOperationsSpec {
 
     }
 
-    predicate valid_state_indices(s: BeaconState, indices: seq<uint64>)
-    {
-        forall i :: 0 <= i < |indices| ==> indices[i] as int < |s.validators|
-    }
     
-    lemma helperIndicesLemma4(s: BeaconState, indices: seq<uint64>, i: nat)
-        requires 0 <= i <= |indices|
-        requires valid_state_indices(s, indices)
-        ensures valid_state_indices(s, indices[..i])
-    {
-        // Thanks Dafny
-    }
-
-    lemma helperIndicesLemma5(indices: seq<uint64>, i: nat)
-        requires i <= |indices|
-        ensures |indices[..i]| == i;
-    {
-        // Thanks Dafny
-    }
-
-    lemma helperIndicesLemma6(indices: seq<uint64>, i: nat)
-        requires i == |indices|
-        ensures indices[..i] == indices
-    {
-        // Thanks Dafny
-    }
-
-    lemma helperIndicesLemma7(indices: seq<uint64>, i: nat)
-        requires i < |indices|
-        ensures indices[..i+1] == indices[..i] + [indices[i]];
-    {
-        // Thanks Dafny
-    }
-
+    
     function updateAttesterSlashing(s: BeaconState, indices: seq<uint64>) : BeaconState 
         
         requires |get_active_validator_indices(s.validators, get_current_epoch(s))| > 0
@@ -1259,731 +755,16 @@ module ProcessOperationsSpec {
             s
     }
 
-
-     
-    // function updateAttesterSlashing(s: BeaconState, indices: seq<ValidatorIndex>) : BeaconState 
-    //     requires forall i :: 0 <= i < |indices| ==> indices[i] as int < |s.validators| 
-    //     requires |get_active_validator_indices(s.validators, get_current_epoch(s))| > 0
-    //     requires |s.validators| == |s.balances|
-
-    //     ensures |s.validators| == |updateAttesterSlashing(s, indices).validators| 
-    //     ensures updateAttesterSlashing(s, indices).slot == s.slot
-
-    //     ensures |updateAttesterSlashing(s, indices).validators| == |updateAttesterSlashing(s, indices).balances|   
-    //     ensures updateAttesterSlashing(s, indices).eth1_deposit_index == s.eth1_deposit_index
-    //     ensures |get_active_validator_indices(updateAttesterSlashing(s, indices).validators, get_current_epoch(updateAttesterSlashing(s, indices)))| > 0
-  
-    //     decreases indices
-    // {
-    //     if |indices| == 0 then 
-    //         s
-    //     else 
-    //         if is_slashable_validator(s.validators[indices[0]], get_current_epoch(s)) then
-    //             slashValidatorPreservesActivateValidators(s, indices[0], get_beacon_proposer_index(s));
-    //             updateAttesterSlashing(slash_validator(s, indices[0], get_beacon_proposer_index(s)), indices[1..])
-    //         else
-    //             updateAttesterSlashing(s, indices[1..])
-    // }
     
-    
-    
-    // function updateAttesterSlashing2(s: BeaconState, a: AttesterSlashing) : BeaconState 
-    //     requires is_slashable_attestation_data(a.attestation_1.data, a.attestation_2.data)
-    //     requires is_valid_indexed_attestation(s, a.attestation_1)
-    //     requires is_valid_indexed_attestation(s, a.attestation_2)
-    //     requires forall i :: 0 <= i < |a.attestation_1.attesting_indices| ==> a.attestation_1.attesting_indices[i] as int < |s.validators|
-    //     requires forall i :: 0 <= i < |a.attestation_2.attesting_indices| ==> a.attestation_2.attesting_indices[i] as int < |s.validators|
-    //     requires |get_active_validator_indices(s.validators, get_current_epoch(s))| > 0
-    //     requires |s.validators| == |s.balances|
-
-    //     ensures |s.validators| == |updateAttesterSlashing(s,a).validators| 
-    //     //ensures updateAttesterSlashing(s, a).slot == s.slot
-    //     //ensures get_current_epoch(s) == get_current_epoch(updateProposerSlashing(s, ps))
-    // {
-    //     var indices := sorted_intersection(a.attestation_1.attesting_indices, a.attestation_2.attesting_indices);
-    //     slashAttesterIndices(s, indices)
-    // }
-
-    // function slashAttesterIndices(s: BeaconState, indices: seq<ValidatorIndex>): BeaconState
-    //     requires forall i :: 0 <= i < |indices| ==> indices[i] as int < |s.validators| 
-    //     requires |get_active_validator_indices(s.validators, get_current_epoch(s))| > 0
-    //     requires |s.validators| == |s.balances|
-    //     ensures |s.validators| == |slashAttesterIndices(s, indices).validators| 
-    //     ensures slashAttesterIndices(s, indices).slot == s.slot
-    //     decreases indices
-    // {
-    //     if |indices| == 0 then 
-    //         s
-    //     else 
-    //         if is_slashable_validator(s.validators[indices[0]], get_current_epoch(s)) then
-    //             slashValidatorPreservesActivateValidators(s, indices[0], get_beacon_proposer_index(s));
-    //             slashAttesterIndices(slash_validator(s, indices[0], get_beacon_proposer_index(s)), indices[1..])
-    //         else
-    //             slashAttesterIndices(s, indices[1..])
-    // }
-
-    /** initiate_validator_exit
-     *  
-     *  Initiate the exit of the validator with index ``index``.
-     *
-     */
-    function method initiate_validator_exit(s: BeaconState, index: ValidatorIndex) : BeaconState
-        requires |s.validators| == |s.balances|
-        requires index as int < |s.validators| 
-        //requires s.validators[index].exitEpoch == FAR_FUTURE_EPOCH
-
-        ensures |s.validators| == |initiate_validator_exit(s,index).validators|
-        ensures |initiate_validator_exit(s,index).validators| == |initiate_validator_exit(s,index).balances|
-        ensures initiate_validator_exit(s,index).validators[index].exitEpoch > get_current_epoch(s) + MAX_SEED_LOOKAHEAD
-                || initiate_validator_exit(s,index).validators[index].exitEpoch == s.validators[index].exitEpoch
-        ensures forall i :: (0 <= i < |s.validators|) && (i != index as int) ==> 
-                initiate_validator_exit(s,index).validators[i].exitEpoch == s.validators[i].exitEpoch
-        ensures initiate_validator_exit(s,index).validators[index].exitEpoch < FAR_FUTURE_EPOCH
-    {
-        // # Return if validator already initiated exit
-        // validator = state.validators[index]
-        if s.validators[index].exitEpoch != FAR_FUTURE_EPOCH then
-            s
-        else 
-        //     return
-        //assert s.validators[index].exitEpoch == FAR_FUTURE_EPOCH;
-        
-        // # Compute exit queue epoch
-        // exit_epochs = [v.exit_epoch for v in state.validators if v.exit_epoch != FAR_FUTURE_EPOCH]
-        var exit_epochs := get_exit_epochs(s.validators);
-        
-        // exit_queue_epoch = max(exit_epochs + [compute_activation_exit_epoch(get_current_epoch(state))])
-        var exit_queue_epoch := max_epoch(exit_epochs + [compute_activation_exit_epoch(get_current_epoch(s))]);
-
-        assert compute_activation_exit_epoch(get_current_epoch(s)) > get_current_epoch(s) + MAX_SEED_LOOKAHEAD;
-        assert compute_activation_exit_epoch(get_current_epoch(s)) in exit_epochs + [compute_activation_exit_epoch(get_current_epoch(s))];
-        assert max_epoch(exit_epochs + [compute_activation_exit_epoch(get_current_epoch(s))]) >= compute_activation_exit_epoch(get_current_epoch(s));
-        assert exit_queue_epoch > get_current_epoch(s) + MAX_SEED_LOOKAHEAD;
-
-        // exit_queue_churn = len([v for v in state.validators if v.exit_epoch == exit_queue_epoch])
-        var exit_queue_churn := |get_queue_churn(s.validators, exit_queue_epoch)|;
-        var validator_churn_limit := get_validator_churn_limit(s);
-
-        // if exit_queue_churn >= get_validator_churn_limit(state):
-        //     exit_queue_epoch += Epoch(1)
-
-        // # Set validator exit epoch and withdrawable epoch
-        // validator.exit_epoch = exit_queue_epoch
-        // validator.withdrawable_epoch = Epoch(validator.exit_epoch + MIN_VALIDATOR_WITHDRAWABILITY_DELAY)
-
-        assume exit_queue_epoch as int + 1 + MIN_VALIDATOR_WITHDRAWABILITY_DELAY as nat < 0x10000000000000000; 
-
-        if exit_queue_churn  >= get_validator_churn_limit(s) as nat then 
-            s.(validators := s.validators[index as int := s.validators[index].(exitEpoch := exit_queue_epoch + 1 as Epoch,
-                                                            withdrawable_epoch := (exit_queue_epoch as nat + 1 + MIN_VALIDATOR_WITHDRAWABILITY_DELAY as nat) as Epoch)])
-        else
-            s.(validators := s.validators[index as int := s.validators[index].(exitEpoch := exit_queue_epoch,
-                                                            withdrawable_epoch := (exit_queue_epoch as nat + MIN_VALIDATOR_WITHDRAWABILITY_DELAY as nat) as Epoch)])
-    }
-
-
-        /** slash_validator
-     *  
-     *  Slash the validator with index ``slashed_index``.
-     */
-    function method slash_validator(s: BeaconState, slashed_index: ValidatorIndex, whistleblower_index: ValidatorIndex): BeaconState
-        requires slashed_index as int < |s.validators| 
-        requires whistleblower_index as int < |s.validators| 
-        requires |s.validators| == |s.balances|
-        //requires s.validators[slashed_index].exitEpoch == FAR_FUTURE_EPOCH
-        requires |get_active_validator_indices(s.validators, get_current_epoch(s))| > 0
-        //ensures |get_active_validator_indices(slash_validator(s,slashed_index,whistleblower_index).validators, get_current_epoch(s))| > 0
-        ensures slash_validator(s, slashed_index, whistleblower_index).slot == s.slot
-    {
-        var epoch : Epoch := get_current_epoch(s);
-        var proposer_index := get_beacon_proposer_index(s);
-
-        var s' := initiate_validator_exit(s, slashed_index); // only validator exitEpoch & withdrawable_epoch fields possibly changed
-
-        assert |s.balances| == |s'.balances|;
-        assert |s'.balances| == |s'.validators|;
-        assert get_current_epoch(s) == get_current_epoch(s');
-        
-        //assert initiate_validator_exit(s,slashed_index).validators[slashed_index].exitEpoch > get_current_epoch(s) + MAX_SEED_LOOKAHEAD;
-        assert forall i :: (0 <= i < |s.validators|) && (i != slashed_index as int) ==> 
-                initiate_validator_exit(s,slashed_index).validators[i].exitEpoch == s.validators[i].exitEpoch;
-        
-        //assert s'.validators[slashed_index].exitEpoch > get_current_epoch(s) + MAX_SEED_LOOKAHEAD;
-        assert forall i :: (0 <= i < |s.validators|) && (i != slashed_index as int) ==> 
-                s'.validators[i].exitEpoch == s.validators[i].exitEpoch;
-        
-        assert forall i :: (0 <= i < |s'.validators|) ==> 
-                is_active_validator(s.validators[i], get_current_epoch(s)) == is_active_validator(s'.validators[i], get_current_epoch(s'));
-
-        initiateValidatorExitPreservesActivateValidators(s.validators, s'.validators,  get_current_epoch(s'));
-        assert get_active_validator_indices(s'.validators, get_current_epoch(s')) == get_active_validator_indices(s.validators, get_current_epoch(s));
-        assert |get_active_validator_indices(s'.validators, get_current_epoch(s'))| > 0;
-        
-        // NOTE:    steps reordered to suit Dafny function method output
-        //          order irrelevant as 'Apply proposer and whistleblower rewards' relies only on s'.validators[slashed_index].effective_balance
-
-        // # Apply proposer and whistleblower rewards
-        
-        // if whistleblower_index is None:
-        //     whistleblower_index = proposer_index
-        // Note: 'None' is not available in Dafny and so functions that call slash_validator will have this parameter set to proposer_index
-        
-        
-        // NOTE: there doesn't seem to be anything to check that the validator being slashed isn't the proposer of the block that contains the ps
-        // though it makes sense that a validator wouldn't proposer to slash itself!
-        // assert slashed_index != whistleblower_index;
-
-        var whistleblower_reward : Gwei := (s'.validators[slashed_index].effective_balance as int / WHISTLEBLOWER_REWARD_QUOTIENT as nat) as Gwei;
-        var proposer_reward := (whistleblower_reward as int / PROPOSER_REWARD_QUOTIENT as int) as Gwei;
-        var validator_penalty := (s'.validators[slashed_index].effective_balance as int / MIN_SLASHING_PENALTY_QUOTIENT as nat) as Gwei;
-
-        //s' := increase_balance(s', proposer_index, proposer_reward);
-        //s' := increase_balance(s', whistleblower_index, Gwei(whistleblower_reward - proposer_reward));
-        
-        //var validator := s'.validators[slashed_index];
-        // validator.slashed = True
-        // validator.withdrawable_epoch = max(validator.withdrawable_epoch, Epoch(epoch + EPOCHS_PER_SLASHINGS_VECTOR))
-        // state.slashings[epoch % EPOCHS_PER_SLASHINGS_VECTOR] += validator.effective_balance
-
-        assume (s'.slashings[epoch as int % EPOCHS_PER_SLASHINGS_VECTOR as nat] as int + s'.validators[slashed_index].effective_balance as int) < 0x10000000000000000;
-        assert slashed_index as int < |s'.balances|; 
-        assert proposer_index as int < |s'.balances|; 
-        assert whistleblower_index as int < |s'.balances|; 
-        assume s'.balances[proposer_index] as int + proposer_reward as int < 0x10000000000000000;
-        // Note: if proposer_index == whistleblower_index then the following assume statement is required rather than
-        // assume s'.balances[whistleblower_index] as int + (whistleblower_reward - proposer_reward) as int < 0x10000000000000000;
-        // The following assume statement covers both cases and will be replaced at a later date by functionality that
-        // takes into account the total amount of Eth available.
-        assume s'.balances[whistleblower_index] as int + whistleblower_reward  as int < 0x10000000000000000;
-
-        s'.(validators := s'.validators[slashed_index := s'.validators[slashed_index].(slashed := true,
-                                                            withdrawable_epoch := max(s'.validators[slashed_index].withdrawable_epoch as nat,(epoch as nat + EPOCHS_PER_SLASHINGS_VECTOR as nat)) as Epoch)],
-            slashings := s'.slashings[(epoch as int % EPOCHS_PER_SLASHINGS_VECTOR as nat) := s'.slashings[epoch as int % EPOCHS_PER_SLASHINGS_VECTOR as nat] + s'.validators[slashed_index].effective_balance],
-            balances := increase_balance(
-                            increase_balance(
-                                decrease_balance(s', slashed_index, validator_penalty), 
-                                proposer_index, 
-                                proposer_reward), 
-                            whistleblower_index, 
-                            (whistleblower_reward - proposer_reward)).balances)
-            
-        
-        // the triple nested mutation of balances is somewhat messy but for the moment it allows slashed_validator to remain as a function method 
-        //(rather than a method)
-
-    }
-
-    lemma slash_validator_lemma(s: BeaconState, slashed_index: ValidatorIndex, whistleblower_index: ValidatorIndex)
-        requires slashed_index as int < |s.validators| 
-        requires whistleblower_index as int < |s.validators| 
-        requires |s.validators| == |s.balances|
-        //requires s.validators[slashed_index].exitEpoch == FAR_FUTURE_EPOCH
-        requires |get_active_validator_indices(s.validators, get_current_epoch(s))| > 0
-        ensures slash_validator(s, slashed_index, whistleblower_index).validators[slashed_index].slashed
-    {
-
-    }
-
-    // ?? prove that the only way slashed is set to true is by calling slash_validator?? 
-    
-    lemma slashValidatorPreservesActivateValidators(s: BeaconState, slashed_index: ValidatorIndex, whistleblower_index: ValidatorIndex)
-        requires slashed_index as int < |s.validators| 
-        requires whistleblower_index as int < |s.validators| 
-        requires |s.validators| == |s.balances|
-        //requires s.validators[slashed_index].exitEpoch == FAR_FUTURE_EPOCH
-        requires |get_active_validator_indices(s.validators, get_current_epoch(s))| > 0
-        
-        ensures get_active_validator_indices(s.validators, get_current_epoch(s)) ==
-                    get_active_validator_indices(slash_validator(s,slashed_index,whistleblower_index).validators, get_current_epoch(s))
-    {
-        
-        var epoch : Epoch := get_current_epoch(s);
-        var proposer_index := get_beacon_proposer_index(s);
-        var s' := initiate_validator_exit(s, slashed_index); // only validator exitEpoch & withdrawable_epoch fields possibly changed
-
-        // show initiate validator exit doesn't change the set of active validator indices
-        
-        assert |s.balances| == |s'.balances|;
-        assert |s'.balances| == |s'.validators|;
-        assert epoch == get_current_epoch(s');
-        
-        //assert initiate_validator_exit(s,slashed_index).validators[slashed_index].exitEpoch > epoch + MAX_SEED_LOOKAHEAD;
-        assert forall i :: (0 <= i < |s.validators|) && (i != slashed_index as int) ==> 
-                initiate_validator_exit(s,slashed_index).validators[i].exitEpoch == s.validators[i].exitEpoch;
-        
-        //assert s'.validators[slashed_index].exitEpoch > epoch + MAX_SEED_LOOKAHEAD;
-        assert forall i :: (0 <= i < |s.validators|) && (i != slashed_index as int) ==> 
-                s'.validators[i].exitEpoch == s.validators[i].exitEpoch;
-        
-        assert forall i :: (0 <= i < |s'.validators|) ==> 
-                is_active_validator(s.validators[i], epoch) == is_active_validator(s'.validators[i], epoch);
-
-        initiateValidatorExitPreservesActivateValidators(s.validators, s'.validators, epoch);
-        assert get_active_validator_indices(s'.validators, epoch) == get_active_validator_indices(s.validators, epoch);
-        assert |get_active_validator_indices(s'.validators, epoch)| > 0;
-
-        // show update to s', including rewards/penalties, doesn't change the set of active validator indices
-        var whistleblower_reward : Gwei := (s'.validators[slashed_index].effective_balance as int / WHISTLEBLOWER_REWARD_QUOTIENT as nat) as Gwei;
-        var proposer_reward := (whistleblower_reward as int / PROPOSER_REWARD_QUOTIENT as int) as Gwei;
-        var validator_penalty := (s'.validators[slashed_index].effective_balance as int / MIN_SLASHING_PENALTY_QUOTIENT as nat) as Gwei;
-
-        assume (s'.slashings[epoch as int % EPOCHS_PER_SLASHINGS_VECTOR as nat] as int + s'.validators[slashed_index].effective_balance as int) < 0x10000000000000000;
-        assert slashed_index as int < |s'.balances|; 
-        assert proposer_index as int < |s'.balances|; 
-        assert whistleblower_index as int < |s'.balances|; 
-        
-        assume s'.balances[proposer_index] as int + proposer_reward as int < 0x10000000000000000;
-        assume s'.balances[whistleblower_index] as int + whistleblower_reward  as int < 0x10000000000000000;
-
-
-        s' := s'.(  validators := s'.validators[slashed_index := s'.validators[slashed_index].(slashed := true,
-                                                            withdrawable_epoch := max(s'.validators[slashed_index].withdrawable_epoch as nat,(epoch as nat + EPOCHS_PER_SLASHINGS_VECTOR as nat)) as Epoch)],
-                    slashings := s'.slashings[(epoch as int % EPOCHS_PER_SLASHINGS_VECTOR as nat) := s'.slashings[epoch as int % EPOCHS_PER_SLASHINGS_VECTOR as nat] + s'.validators[slashed_index].effective_balance],
-                    balances := increase_balance(
-                                    increase_balance(
-                                        decrease_balance(s', slashed_index, validator_penalty), 
-                                        proposer_index, 
-                                        proposer_reward), 
-                                    whistleblower_index, 
-                                    (whistleblower_reward - proposer_reward)).balances);
-        
-        //assert s'.validators[slashed_index].exitEpoch > epoch + MAX_SEED_LOOKAHEAD;
-        assert forall i :: (0 <= i < |s.validators|) && (i != slashed_index as int) ==> 
-                s'.validators[i].exitEpoch == s.validators[i].exitEpoch;
-
-        assert forall i :: (0 <= i < |s'.validators|) ==> 
-                is_active_validator(s.validators[i], epoch) == is_active_validator(s'.validators[i], epoch);
-
-        assert s' == slash_validator(s,slashed_index,whistleblower_index);
-        
-        sameActiveValidatorsImpliesSameActiveValidatorIndices(s.validators, s'.validators, epoch);
-        assert get_active_validator_indices(s'.validators, epoch) == get_active_validator_indices(s.validators, epoch);
-    }
-
- 
-    
-    function method get_exit_epochs(sv: ListOfValidators) : seq<Epoch>
-        ensures forall i :: 0 <= i < |get_exit_epochs(sv)| ==> get_exit_epochs(sv)[i] < FAR_FUTURE_EPOCH
-    {
-        if |sv| == 0 
-            then []
-        else 
-            if sv[0].exitEpoch != FAR_FUTURE_EPOCH 
-                then [sv[0].exitEpoch] + get_exit_epochs(sv[1..])
-                else get_exit_epochs(sv[1..])
-    }
-
-    function method get_queue_churn(sv: ListOfValidators, exit_queue_epoch: Epoch) : seq<Validator>
-    {
-        if |sv| == 0 
-            then []
-        else 
-            if sv[0].exitEpoch == exit_queue_epoch 
-                then [sv[0]] + get_queue_churn(sv[1..], exit_queue_epoch)
-                else get_queue_churn(sv[1..], exit_queue_epoch)
-    }
-
-    // // Check if ``validator`` is active.
-    // predicate method is_active_validator(validator: Validator, epoch: Epoch)
-    // {
-    //     validator.activation_epoch <= epoch < validator.exitEpoch
-    // }
-
-    // // Return the sequence of active validator indices at ``epoch``.
-    // // function get_active_validator_indices(s: BeaconState, epoch: Epoch) : seq<ValidatorIndex>
-    // // NOTE: as BeaconState isn't modified and only validators field is accessed, the function is better suited to 
-    // //      using an input parameter of just the list of validators (rather than the entire state)
-    // function method get_active_validator_indices(sv: ListOfValidators, epoch: Epoch) : seq<ValidatorIndex>
-    //     ensures |get_active_validator_indices(sv,epoch)| <= |sv|
-    // {
-    //     //[ValidatorIndex(i) for i, v in enumerate(state.validators) if is_active_validator(v, epoch)]
-    //     if |sv| == 0 then []
-    //     else 
-    //         if is_active_validator(sv[|sv|-1], epoch) then get_active_validator_indices(sv[..|sv|-1], epoch) + [(|sv|-1) as ValidatorIndex]
-    //         else get_active_validator_indices(sv[..|sv|-1], epoch)
-    // }
-
-    //Return the validator churn limit for the current epoch.
-    function method get_validator_churn_limit(s: BeaconState) : uint64
-        //ensures MIN_PER_EPOCH_CHURN_LIMIT <= get_validator_churn_limit(s) <= 
-        //    (|get_active_validator_indices(s.validators, get_current_epoch(s))| as uint64/CHURN_LIMIT_QUOTIENT)  // i.e. at least 4
-    {
-        var active_validator_indices := get_active_validator_indices(s.validators, get_current_epoch(s));
-        max(MIN_PER_EPOCH_CHURN_LIMIT as nat, (|active_validator_indices| as uint64/CHURN_LIMIT_QUOTIENT) as nat) as uint64
-    }
-
-
-    
-    function method max_epoch(se: seq<Epoch>): Epoch
-        requires |se| > 0
-        ensures forall i :: 0 <= i < |se| ==> max_epoch(se) >= se[i]
-        decreases se
-    {
-        if |se| == 1 then se[0]
-        else
-            if se[0] > max_epoch(se[1..]) then se[0]
-            else max_epoch(se[1..])
-    }
-    
-    // Return the epoch during which validator activations and exits initiated in ``epoch`` take effect.
-    function method compute_activation_exit_epoch(epoch: Epoch) : Epoch
-        requires epoch as int + 1 + MAX_SEED_LOOKAHEAD as int < 0x10000000000000000 
-        ensures compute_activation_exit_epoch(epoch) > epoch
-    {
-        epoch + 1 as Epoch + MAX_SEED_LOOKAHEAD as Epoch
-    }
-
-    // //Return the randao mix at a recent ``epoch``.
-    // function method get_randao_mix(state: BeaconState, epoch: Epoch): Bytes32
-    // {
-    //     state.randao_mixes[epoch % EPOCHS_PER_HISTORICAL_VECTOR as uint64]
-    // }
-
-
-    // // Return the seed at ``epoch``.
-    // function method get_seed(state: BeaconState, epoch: Epoch, domain_type: DomainType): Bytes32
-    //     requires epoch as int + EPOCHS_PER_HISTORICAL_VECTOR - MIN_SEED_LOOKAHEAD  - 1 < 0x10000000000000000
-    // {
-    //     var mix := get_randao_mix(state, (epoch as int + EPOCHS_PER_HISTORICAL_VECTOR - MIN_SEED_LOOKAHEAD - 1) as uint64);  // Avoid underflow
-    //     var sb := serialise(domain_type) + serialise(Uint64(epoch as nat)) + serialise(mix);
-    //     hash(sb)
-    // }
-    
-
-    //Return from ``indices`` a random index sampled by effective balance.
-    function method compute_proposer_index(state: BeaconState, indices: seq<ValidatorIndex>, seed: Bytes32) : ValidatorIndex
-        requires |indices| > 0
-    {
-        // assert len(indices) > 0
-
-        var MAX_RANDOM_BYTE := TWO_UP_8 - 1;
-        var i : uint64 := 0;
-        var total := |indices|;
-        //while true {
-        //     candidate_index = indices[compute_shuffled_index(i % total, total, seed)]
-        //     random_byte = hash(seed + uint_to_bytes(uint64(i // 32)))[i % 32]
-        //     effective_balance = state.validators[candidate_index].effective_balance
-        //     if effective_balance * MAX_RANDOM_BYTE >= MAX_EFFECTIVE_BALANCE * random_byte:
-        //         return candidate_index
-        //    i := i + 1;
-        //}
-        
-        
-        0 as ValidatorIndex // temporary return value
-    }
-
-    // Return the shuffled index corresponding to ``seed`` (and ``index_count``).
-    // Swap or not (https://link.springer.com/content/pdf/10.1007%2F978-3-642-32009-5_1.pdf)
-    // See the 'generalized domain' algorithm on page 3
-    function method compute_shuffled_index(index: uint64, index_count: uint64, seed: Bytes32): ValidatorIndex
-        requires index < index_count
-    {
-        // for current_round in range(SHUFFLE_ROUND_COUNT):
-        //     pivot = bytes_to_uint64(hash(seed + uint_to_bytes(uint8(current_round)))[0:8]) % index_count
-        //     flip = (pivot + index_count - index) % index_count
-        //     position = max(index, flip)
-        //     source = hash(
-        //         seed
-        //         + uint_to_bytes(uint8(current_round))
-        //         + uint_to_bytes(uint32(position // 256))
-        //     )
-        //     byte = uint8(source[(position % 256) // 8])
-        //     bit = (byte >> (position % 8)) % 2
-        //     index = flip if bit else index
-
-        // return index
-
-        0 as ValidatorIndex // temporary return value
-
-    }
-
-    //Return the beacon proposer index at the current slot.
-    function method get_beacon_proposer_index(state: BeaconState): ValidatorIndex
-        requires |get_active_validator_indices(state.validators, get_current_epoch(state))| > 0
-        //ensures is_active_validator(state.validators[get_beacon_proposer_index(state)], get_current_epoch(state))
-    {
-        var epoch := get_current_epoch(state);
-        var seed := hash(serialise(get_seed(state, epoch, DOMAIN_BEACON_PROPOSER)) + serialise(Uint64(state.slot as nat)));
-        var indices := get_active_validator_indices(state.validators, epoch);
-
-        compute_proposer_index(state, indices, seed)
-    }
-
-    // is_slashable_attestation_data
-    // Check if ``data_1`` and ``data_2`` are slashable according to Casper FFG rules.
-    predicate method is_slashable_attestation_data(data_1: AttestationData, data_2: AttestationData)
-    {
-        // Double vote
-        (data_1 != data_2 && data_1.target.epoch == data_2.target.epoch) ||
-        // Surround vote
-        (data_1.source.epoch < data_2.source.epoch && data_2.target.epoch < data_1.target.epoch)
-    }
-
-    // is_valid_indexed_attestation
-    // Check if ``indexed_attestation`` is not empty, has sorted and unique indices and has a valid aggregate signature.
-    // Note: at this time only the first part of the check is being implemented
-
-    lemma valid_indexed_attestation_lemma(s: BeaconState, s': BeaconState, indexed_attestation: IndexedAttestation)
-        requires is_valid_indexed_attestation(s,indexed_attestation) 
-        ensures is_valid_indexed_attestation(s',indexed_attestation)
-    {
-        // Thanks Dafny
-    }
-
-    predicate method is_valid_indexed_attestation(s: BeaconState, indexed_attestation: IndexedAttestation)
-    {
-        // Verify indices are sorted and unique
-        var indices := indexed_attestation.attesting_indices;
-        //if len(indices) == 0 or not indices == sorted(set(indices)):
-        if (|indices| == 0 || !is_attesting_indices_sorted_and_unique(indices))
-            then false
-        else 
-            true
-
-        // Verify aggregate signature, not implemented at this time
-
-        // pubkeys = [state.validators[i].pubkey for i in indices]
-        // domain = get_domain(state, DOMAIN_BEACON_ATTESTER, indexed_attestation.data.target.epoch)
-        // signing_root = compute_signing_root(indexed_attestation.data, domain)
-        // return bls.FastAggregateVerify(pubkeys, signing_root, indexed_attestation.signature)
-    }
-
-    predicate method is_attesting_indices_sorted_and_unique(indices: AttestingIndices)
-        requires |indices| > 0
-    {
-        forall i,j :: 0 <= i < j < |indices| ==> indices[i] < indices[j]
-    }
-
-    
-    lemma initiateValidatorExitPreservesActivateValidators(sv: ListOfValidators, sv': ListOfValidators, epoch: Epoch)
-        requires |sv| == |sv'|
-        requires forall i :: (0 <= i < |sv'|) ==> 
-                is_active_validator(sv[i], epoch) == is_active_validator(sv'[i], epoch)
-        ensures get_active_validator_indices(sv', epoch) == get_active_validator_indices(sv, epoch)
-    {
-        if |sv'| == 0 {
-            assert get_active_validator_indices(sv', epoch) == get_active_validator_indices(sv, epoch);
-        }
-        else {
-            assert get_active_validator_indices(sv', epoch) == 
-                if is_active_validator(sv'[|sv'|-1], epoch) then 
-                    get_active_validator_indices(sv'[..|sv'|-1], epoch) + [(|sv'|-1) as ValidatorIndex]
-                else 
-                    get_active_validator_indices(sv'[..|sv'|-1], epoch);
-            
-            assert get_active_validator_indices(sv', epoch) == 
-                if is_active_validator(sv[|sv|-1], epoch) then 
-                    get_active_validator_indices(sv'[..|sv'|-1], epoch) + [(|sv'|-1) as ValidatorIndex]
-                else 
-                    get_active_validator_indices(sv'[..|sv'|-1], epoch);
-
-            assert |sv| == |sv'|;
-            assert get_active_validator_indices(sv', epoch) == 
-                if is_active_validator(sv[|sv|-1], epoch) then 
-                    get_active_validator_indices(sv'[..|sv|-1], epoch) + [(|sv|-1) as ValidatorIndex]
-                else 
-                    get_active_validator_indices(sv'[..|sv|-1], epoch);
-            initiateValidatorExitPreservesActivateValidators(sv[..|sv|-1], sv'[..|sv|-1], epoch);
-        }
-    }
-
-    
-    lemma sameActiveValidatorsImpliesSameActiveValidatorIndices(sv1: ListOfValidators, sv2: ListOfValidators, epoch: Epoch)
-        requires |sv1| == |sv2|   
-        requires forall i :: (0 <= i < |sv1|) ==> is_active_validator(sv1[i], epoch) == is_active_validator(sv2[i], epoch)
-        ensures get_active_validator_indices(sv1, epoch) == get_active_validator_indices(sv2, epoch)
-    {
-        if |sv1| == 0 {
-            assert get_active_validator_indices(sv2, epoch) == get_active_validator_indices(sv1, epoch);
-        }
-        else {
-            sameActiveValidatorsImpliesSameActiveValidatorIndices(sv1[..|sv1|-1], sv2[..|sv2|-1], epoch);
-        }
-    }
 
     
     
 
 
-    // Beacon State Mutators
-
-    /** increase_balance
-     *  Increase the validator balance at index ``index`` by ``delta``.
-     *
-     *  @notes  The datatype Gwei has temporarily been changed from uint64 to nat so as to simplify the
-     *          properties required to process a deposit. Hence a further requires will be needed to prevent
-     *          overflow once this temporary simplification is removed.
-     *  
-     **/
-    // function method increase_balance(s: BeaconState, index: ValidatorIndex, delta: Gwei): BeaconState 
-    //     requires index as int < |s.balances| 
-    //     requires s.balances[index] as int + delta as int < 0x10000000000000000
-    //     ensures |s.balances| == |increase_balance(s,index,delta).balances|
-    //     ensures increase_balance(s,index,delta).balances[index] == s.balances[index] + delta
-    // {
-    //     s.(
-    //         balances := s.balances[index as int := (s.balances[index] + delta)]
-    //     )
-    // }
+   
+    
 
     
-lemma individualBalanceBoundMaintained(sb: seq<Gwei>, d: Deposit)
-        requires total_balances(sb) + d.data.amount as int < 0x10000000000000000
-        ensures forall i :: 0 <= i < |sb| ==> sb[i] as int + d.data.amount as int < 0x10000000000000000
-    {
-        if |sb| == 0 {
-            // Thanks Dafny
-        }
-        else {
-            assert total_balances(sb) == sb[0] as int + total_balances(sb[1..]);
-            assert sb[0] as int + d.data.amount as int < 0x10000000000000000;
-            assert total_balances(sb[1..]) + d.data.amount as int < 0x10000000000000000;
-            individualBalanceBoundMaintained(sb[1..],d);
-        }
-    } 
-
-    lemma updateBalTotalBySingleDeposit(s: BeaconState, d: Deposit)
-        requires s.eth1_deposit_index as int +  1 < 0x10000000000000000 
-        requires |s.validators| == |s.balances|
-        requires |s.validators| + 1 <= VALIDATOR_REGISTRY_LIMIT as int
-        requires total_balances(s.balances) + d.data.amount as int < 0x10000000000000000
-        
-        ensures total_balances(updateDeposit(s,d).balances) == total_balances(s.balances) + d.data.amount as int < 0x10000000000000000
-        //ensures total_balances(updateDeposit(s,d).balances) == total_balances(s.balances) + total_deposits([d]) 
-    {
-        var pk := seqKeysInValidators(s.validators); 
-        if |s.balances| == 0 {
-            // Thanks Dafny
-        }
-        else {
-            if d.data.pubkey in pk {
-                var index := get_validator_index(pk, d.data.pubkey);
-                individualBalanceBoundMaintained(s.balances,d);
-                //assert updateDeposit(s,d).balances ==  increase_balance(s,index,d.data.amount).balances;
-                //assert increase_balance(s,index,d.data.amount).balances[index] == s.balances[index] + d.data.amount;
-                //assert forall i :: 0 <= i < |s.balances| && i != index as int ==> increase_balance(s,index,d.data.amount).balances[i] == s.balances[i];
-                //assert total_balances(updateDeposit(s,d).balances) == total_balances(increase_balance(s,index,d.data.amount).balances) ;
-                updateExistingBalance(s, index, d.data.amount);
-                //assert total_balances(updateDeposit(s,d).balances) == total_balances(s.balances) + d.data.amount as int ;
-            }
-            else {
-                //assert updateDeposit(s,d).balances == s.balances + [d.data.amount];
-                distBalancesProp(s.balances,[d.data.amount]);
-                //assert total_balances(s.balances + [d.data.amount]) == total_balances(s.balances) + total_balances([d.data.amount]);
-            }
-        }
-    }
-
-    lemma updateExistingBalance(s: BeaconState, index: ValidatorIndex, delta: Gwei)
-        requires index as int < |s.balances| 
-        requires s.balances[index] as int + delta as int < 0x10000000000000000
-        requires |s.balances| < VALIDATOR_REGISTRY_LIMIT as int
-
-        ensures total_balances(increase_balance(s,index,delta).balances) == total_balances(s.balances) + delta as int
-    {
-        //assert increase_balance(s,index,delta).balances[index] == s.balances[index] + delta;
-        //assert forall i :: 0 <= i < |s.balances| && i != index as int ==> increase_balance(s,index,delta).balances[i] == s.balances[i];
-
-        if index as int < |s.balances|-1 {
-            assert increase_balance(s,index,delta).balances == increase_balance(s,index,delta).balances[..index] + [increase_balance(s,index,delta).balances[index]] + increase_balance(s,index,delta).balances[(index+1)..];
-                                                                
-            //assert total_balances(increase_balance(s,index,delta).balances[..index]) == total_balances(s.balances[..index]);
-            //assert total_balances([increase_balance(s,index,delta).balances[index]]) == total_balances([s.balances[index]]) + delta as int;
-            //assert total_balances(increase_balance(s,index,delta).balances[(index+1)..]) == total_balances(s.balances[(index+1)..]);
-
-            //assert total_balances(increase_balance(s,index,delta).balances) == total_balances(increase_balance(s,index,delta).balances[..index] + [increase_balance(s,index,delta).balances[index]] + increase_balance(s,index,delta).balances[(index+1)..]);
-
-            distBalancesProp(increase_balance(s,index,delta).balances[..index], [increase_balance(s,index,delta).balances[index]]);
-            //assert total_balances(increase_balance(s,index,delta).balances[..index] + [increase_balance(s,index,delta).balances[index]]) == total_balances(increase_balance(s,index,delta).balances[..index]) + total_balances([increase_balance(s,index,delta).balances[index]]);
-            distBalancesProp(increase_balance(s,index,delta).balances[..index]+[increase_balance(s,index,delta).balances[index]], increase_balance(s,index,delta).balances[(index+1)..]);
-            //assert total_balances(increase_balance(s,index,delta).balances[..index] + [increase_balance(s,index,delta).balances[index]] + increase_balance(s,index,delta).balances[(index+1)..]) == total_balances(increase_balance(s,index,delta).balances[..index]) + total_balances([increase_balance(s,index,delta).balances[index]]) + total_balances(increase_balance(s,index,delta).balances[index+1..]);
-
-            //assert total_balances(increase_balance(s,index,delta).balances) == total_balances(increase_balance(s,index,delta).balances[..index]) + total_balances([increase_balance(s,index,delta).balances[index]]) + total_balances(increase_balance(s,index,delta).balances[index+1..]);
-            //assert total_balances(increase_balance(s,index,delta).balances) == total_balances(s.balances[..index]) + total_balances([s.balances[index]]) + delta as int + total_balances(s.balances[(index+1)..]);
-
-            //assert total_balances(increase_balance(s,index,delta).balances) == total_balances(s.balances[..index]) + total_balances([s.balances[index]]) + total_balances(s.balances[(index+1)..]) + delta as int;
-
-            assert s.balances == s.balances[..index] + [s.balances[index]] + s.balances[(index+1)..];
-            //assert total_balances(s.balances) == total_balances(s.balances[..index] + [s.balances[index]] + s.balances[(index+1)..]);
-
-            distBalancesProp(s.balances[..index], [s.balances[index]]);
-            //assert total_balances(s.balances[..index] + [s.balances[index]]) == total_balances(s.balances[..index]) + total_balances([s.balances[index]]);
-            distBalancesProp(s.balances[..index]+[s.balances[index]], s.balances[(index+1)..]);
-            //assert total_balances(s.balances[..index] + [s.balances[index]] + s.balances[(index+1)..]) == total_balances(s.balances[..index]) + total_balances([s.balances[index]]) + total_balances(s.balances[index+1..]);
-
-            //assert total_balances(increase_balance(s,index,delta).balances) == total_balances(s.balances) + delta as int;
-        }
-        else {
-            //assert index as int == |s.balances| - 1;
-            assert increase_balance(s,index,delta).balances == increase_balance(s,index,delta).balances[..index] + [increase_balance(s,index,delta).balances[index]];
-                                                                
-            //assert total_balances(increase_balance(s,index,delta).balances[..index]) == total_balances(s.balances[..index]);
-            //assert total_balances([increase_balance(s,index,delta).balances[index]]) == total_balances([s.balances[index]]) + delta as int;
-            
-            //assert total_balances(increase_balance(s,index,delta).balances) == total_balances(increase_balance(s,index,delta).balances[..index] + [increase_balance(s,index,delta).balances[index]]);
-
-            distBalancesProp(increase_balance(s,index,delta).balances[..index], [increase_balance(s,index,delta).balances[index]]);
-            //assert total_balances(increase_balance(s,index,delta).balances[..index] + [increase_balance(s,index,delta).balances[index]]) == total_balances(increase_balance(s,index,delta).balances[..index]) + total_balances([increase_balance(s,index,delta).balances[index]]);
-            
-            
-            //assert total_balances(increase_balance(s,index,delta).balances) == total_balances(s.balances[..index]) + total_balances([s.balances[index]]) + delta as int;
-
-            assert s.balances == s.balances[..index] + [s.balances[index]] ;
-            //assert total_balances(s.balances) == total_balances(s.balances[..index] + [s.balances[index]]);
-
-            distBalancesProp(s.balances[..index], [s.balances[index]]);
-            //assert total_balances(s.balances[..index] + [s.balances[index]]) == total_balances(s.balances[..index]) + total_balances([s.balances[index]]);
-            
-            //assert total_balances(increase_balance(s,index,delta).balances) == total_balances(s.balances) + delta as int;
-        }
-    }
-
-    lemma distBalancesProp(sb1: seq<Gwei>, sb2: seq<Gwei>)
-        ensures total_balances(sb1 + sb2) == total_balances(sb1) + total_balances(sb2) 
-    {
-        if |sb1| == 0 {
-            assert sb1 + sb2 == sb2;
-        }
-        else {
-            var sb := sb1 + sb2;
-            //assert sb == [sb1[0]] +  sb1[1..] + sb2;
-            assert sb[1..] == sb1[1..] + sb2;
-            assert total_balances(sb) == sb[0] as int + total_balances(sb[1..]);
-            //assert total_balances(sb1 + sb2) == sb[0] as int + total_balances(sb1[1..] + sb2);
-            distBalancesProp(sb1[1..],sb2);
-
-        }
-    }
-
-    lemma distDepositsProp(sd1: seq<Deposit>, sd2: seq<Deposit>)
-        ensures total_deposits(sd1 + sd2) == total_deposits(sd1) + total_deposits(sd2) 
-    {
-        if |sd2| == 0 {
-            assert sd1 + sd2 == sd1;
-        }
-        else {
-            var sd := sd1 + sd2;
-            //assert sd == sd1 + sd2[..|sd2|-1] +  [sd2[|sd2|-1]];
-            assert sd[..|sd|-1] == sd1 + sd2[..|sd2|-1] ;
-            assert total_deposits(sd) == total_deposits(sd[..|sd|-1]) + sd2[|sd2|-1].data.amount as int;
-            //assert total_deposits(sd1 + sd2) == total_deposits(sd1 + sd2[..|sd2|-1] ) + sd2[|sd2|-1].data.amount as int;
-            distDepositsProp(sd1, sd2[..|sd2|-1] );
-        }
-    }
-    lemma subsetDepositSumProp(deposits: seq<Deposit>, i: nat)
-        requires i <= |deposits|
-        ensures total_deposits(deposits[..i]) <= total_deposits(deposits);
-    {
-        if i == |deposits| {
-            assert deposits[..i] == deposits;
-        }
-        else {
-            //assert i < |deposits|;
-            assert deposits == deposits[..i] + deposits[i..];
-            assert total_deposits(deposits) == total_deposits(deposits[..i] + deposits[i..]);
-            distDepositsProp(deposits[..i], deposits[i..]);
-            //assert total_deposits(deposits[..i] + deposits[i..]) == total_deposits(deposits[..i]) + total_deposits(deposits[i..]); 
-        }
-    }
+    
 
 }
