src/dafny/beacon/Helpers.p.dfy
@@ -195,4 +195,316 @@ module BeaconHelperProofs {
             ==> len_indices * ((slot * CPS + cIndex) + 1) / (CPS * SLOTS_PER_EPOCH as nat) > len_indices * (slot * CPS + cIndex) / (CPS * SLOTS_PER_EPOCH as nat);
     }
 
+
+ 
+    lemma slash_validator_lemma(s: BeaconState, slashed_index: ValidatorIndex, whistleblower_index: ValidatorIndex)
+        requires slashed_index as int < |s.validators| 
+        requires whistleblower_index as int < |s.validators| 
+        requires |s.validators| == |s.balances|
+        //requires s.validators[slashed_index].exitEpoch == FAR_FUTURE_EPOCH
+        requires |get_active_validator_indices(s.validators, get_current_epoch(s))| > 0
+        ensures slash_validator(s, slashed_index, whistleblower_index).validators[slashed_index].slashed
+    {
+
+    }
+
+    // ?? prove that the only way slashed is set to true is by calling slash_validator?? 
+    
+    lemma slashValidatorPreservesActivateValidators(s: BeaconState, slashed_index: ValidatorIndex, whistleblower_index: ValidatorIndex)
+        requires slashed_index as int < |s.validators| 
+        requires whistleblower_index as int < |s.validators| 
+        requires |s.validators| == |s.balances|
+        //requires s.validators[slashed_index].exitEpoch == FAR_FUTURE_EPOCH
+        requires |get_active_validator_indices(s.validators, get_current_epoch(s))| > 0
+        
+        ensures get_active_validator_indices(s.validators, get_current_epoch(s)) ==
+                    get_active_validator_indices(slash_validator(s,slashed_index,whistleblower_index).validators, get_current_epoch(s))
+    {
+        
+        var epoch : Epoch := get_current_epoch(s);
+        var proposer_index := get_beacon_proposer_index(s);
+        var s' := initiate_validator_exit(s, slashed_index); // only validator exitEpoch & withdrawable_epoch fields possibly changed
+
+        // show initiate validator exit doesn't change the set of active validator indices
+        
+        assert |s.balances| == |s'.balances|;
+        assert |s'.balances| == |s'.validators|;
+        assert epoch == get_current_epoch(s');
+        
+        //assert initiate_validator_exit(s,slashed_index).validators[slashed_index].exitEpoch > epoch + MAX_SEED_LOOKAHEAD;
+        assert forall i :: (0 <= i < |s.validators|) && (i != slashed_index as int) ==> 
+                initiate_validator_exit(s,slashed_index).validators[i].exitEpoch == s.validators[i].exitEpoch;
+        
+        //assert s'.validators[slashed_index].exitEpoch > epoch + MAX_SEED_LOOKAHEAD;
+        assert forall i :: (0 <= i < |s.validators|) && (i != slashed_index as int) ==> 
+                s'.validators[i].exitEpoch == s.validators[i].exitEpoch;
+        
+        assert forall i :: (0 <= i < |s'.validators|) ==> 
+                is_active_validator(s.validators[i], epoch) == is_active_validator(s'.validators[i], epoch);
+
+        initiateValidatorExitPreservesActivateValidators(s.validators, s'.validators, epoch);
+        assert get_active_validator_indices(s'.validators, epoch) == get_active_validator_indices(s.validators, epoch);
+        assert |get_active_validator_indices(s'.validators, epoch)| > 0;
+
+        // show update to s', including rewards/penalties, doesn't change the set of active validator indices
+        var whistleblower_reward : Gwei := (s'.validators[slashed_index].effective_balance as int / WHISTLEBLOWER_REWARD_QUOTIENT as nat) as Gwei;
+        var proposer_reward := (whistleblower_reward as int / PROPOSER_REWARD_QUOTIENT as int) as Gwei;
+        var validator_penalty := (s'.validators[slashed_index].effective_balance as int / MIN_SLASHING_PENALTY_QUOTIENT as nat) as Gwei;
+
+        assume (s'.slashings[epoch as int % EPOCHS_PER_SLASHINGS_VECTOR as nat] as int + s'.validators[slashed_index].effective_balance as int) < 0x10000000000000000;
+        assert slashed_index as int < |s'.balances|; 
+        assert proposer_index as int < |s'.balances|; 
+        assert whistleblower_index as int < |s'.balances|; 
+        
+        assume s'.balances[proposer_index] as int + proposer_reward as int < 0x10000000000000000;
+        assume s'.balances[whistleblower_index] as int + whistleblower_reward  as int < 0x10000000000000000;
+
+
+        s' := s'.(  validators := s'.validators[slashed_index := s'.validators[slashed_index].(slashed := true,
+                                                            withdrawable_epoch := max(s'.validators[slashed_index].withdrawable_epoch as nat,(epoch as nat + EPOCHS_PER_SLASHINGS_VECTOR as nat)) as Epoch)],
+                    slashings := s'.slashings[(epoch as int % EPOCHS_PER_SLASHINGS_VECTOR as nat) := s'.slashings[epoch as int % EPOCHS_PER_SLASHINGS_VECTOR as nat] + s'.validators[slashed_index].effective_balance],
+                    balances := increase_balance(
+                                    increase_balance(
+                                        decrease_balance(s', slashed_index, validator_penalty), 
+                                        proposer_index, 
+                                        proposer_reward), 
+                                    whistleblower_index, 
+                                    (whistleblower_reward - proposer_reward)).balances);
+        
+        //assert s'.validators[slashed_index].exitEpoch > epoch + MAX_SEED_LOOKAHEAD;
+        assert forall i :: (0 <= i < |s.validators|) && (i != slashed_index as int) ==> 
+                s'.validators[i].exitEpoch == s.validators[i].exitEpoch;
+
+        assert forall i :: (0 <= i < |s'.validators|) ==> 
+                is_active_validator(s.validators[i], epoch) == is_active_validator(s'.validators[i], epoch);
+
+        assert s' == slash_validator(s,slashed_index,whistleblower_index);
+        
+        sameActiveValidatorsImpliesSameActiveValidatorIndices(s.validators, s'.validators, epoch);
+        assert get_active_validator_indices(s'.validators, epoch) == get_active_validator_indices(s.validators, epoch);
+    }
+
+
+    // is_valid_indexed_attestation
+    // Check if ``indexed_attestation`` is not empty, has sorted and unique indices and has a valid aggregate signature.
+    // Note: at this time only the first part of the check is being implemented
+
+    lemma valid_indexed_attestation_lemma(s: BeaconState, s': BeaconState, indexed_attestation: IndexedAttestation)
+        requires is_valid_indexed_attestation(s,indexed_attestation) 
+        ensures is_valid_indexed_attestation(s',indexed_attestation)
+    {
+        // Thanks Dafny
+    }
+
+    lemma initiateValidatorExitPreservesActivateValidators(sv: ListOfValidators, sv': ListOfValidators, epoch: Epoch)
+        requires |sv| == |sv'|
+        requires forall i :: (0 <= i < |sv'|) ==> 
+                is_active_validator(sv[i], epoch) == is_active_validator(sv'[i], epoch)
+        ensures get_active_validator_indices(sv', epoch) == get_active_validator_indices(sv, epoch)
+    {
+        if |sv'| == 0 {
+            assert get_active_validator_indices(sv', epoch) == get_active_validator_indices(sv, epoch);
+        }
+        else {
+            assert get_active_validator_indices(sv', epoch) == 
+                if is_active_validator(sv'[|sv'|-1], epoch) then 
+                    get_active_validator_indices(sv'[..|sv'|-1], epoch) + [(|sv'|-1) as ValidatorIndex]
+                else 
+                    get_active_validator_indices(sv'[..|sv'|-1], epoch);
+            
+            assert get_active_validator_indices(sv', epoch) == 
+                if is_active_validator(sv[|sv|-1], epoch) then 
+                    get_active_validator_indices(sv'[..|sv'|-1], epoch) + [(|sv'|-1) as ValidatorIndex]
+                else 
+                    get_active_validator_indices(sv'[..|sv'|-1], epoch);
+
+            assert |sv| == |sv'|;
+            assert get_active_validator_indices(sv', epoch) == 
+                if is_active_validator(sv[|sv|-1], epoch) then 
+                    get_active_validator_indices(sv'[..|sv|-1], epoch) + [(|sv|-1) as ValidatorIndex]
+                else 
+                    get_active_validator_indices(sv'[..|sv|-1], epoch);
+            initiateValidatorExitPreservesActivateValidators(sv[..|sv|-1], sv'[..|sv|-1], epoch);
+        }
+    }
+
+    
+    lemma sameActiveValidatorsImpliesSameActiveValidatorIndices(sv1: ListOfValidators, sv2: ListOfValidators, epoch: Epoch)
+        requires |sv1| == |sv2|   
+        requires forall i :: (0 <= i < |sv1|) ==> is_active_validator(sv1[i], epoch) == is_active_validator(sv2[i], epoch)
+        ensures get_active_validator_indices(sv1, epoch) == get_active_validator_indices(sv2, epoch)
+    {
+        if |sv1| == 0 {
+            assert get_active_validator_indices(sv2, epoch) == get_active_validator_indices(sv1, epoch);
+        }
+        else {
+            sameActiveValidatorsImpliesSameActiveValidatorIndices(sv1[..|sv1|-1], sv2[..|sv2|-1], epoch);
+        }
+    }
+
+    lemma individualBalanceBoundMaintained(sb: seq<Gwei>, d: Deposit)
+        requires total_balances(sb) + d.data.amount as int < 0x10000000000000000
+        ensures forall i :: 0 <= i < |sb| ==> sb[i] as int + d.data.amount as int < 0x10000000000000000
+    {
+        if |sb| == 0 {
+            // Thanks Dafny
+        }
+        else {
+            assert total_balances(sb) == sb[0] as int + total_balances(sb[1..]);
+            assert sb[0] as int + d.data.amount as int < 0x10000000000000000;
+            assert total_balances(sb[1..]) + d.data.amount as int < 0x10000000000000000;
+            individualBalanceBoundMaintained(sb[1..],d);
+        }
+    } 
+
+    lemma updateBalTotalBySingleDeposit(s: BeaconState, d: Deposit)
+        requires s.eth1_deposit_index as int +  1 < 0x10000000000000000 
+        requires |s.validators| == |s.balances|
+        requires |s.validators| + 1 <= VALIDATOR_REGISTRY_LIMIT as int
+        requires total_balances(s.balances) + d.data.amount as int < 0x10000000000000000
+        
+        ensures total_balances(updateDeposit(s,d).balances) == total_balances(s.balances) + d.data.amount as int < 0x10000000000000000
+        //ensures total_balances(updateDeposit(s,d).balances) == total_balances(s.balances) + total_deposits([d]) 
+    {
+        var pk := seqKeysInValidators(s.validators); 
+        if |s.balances| == 0 {
+            // Thanks Dafny
+        }
+        else {
+            if d.data.pubkey in pk {
+                var index := get_validator_index(pk, d.data.pubkey);
+                individualBalanceBoundMaintained(s.balances,d);
+                //assert updateDeposit(s,d).balances ==  increase_balance(s,index,d.data.amount).balances;
+                //assert increase_balance(s,index,d.data.amount).balances[index] == s.balances[index] + d.data.amount;
+                //assert forall i :: 0 <= i < |s.balances| && i != index as int ==> increase_balance(s,index,d.data.amount).balances[i] == s.balances[i];
+                //assert total_balances(updateDeposit(s,d).balances) == total_balances(increase_balance(s,index,d.data.amount).balances) ;
+                updateExistingBalance(s, index, d.data.amount);
+                //assert total_balances(updateDeposit(s,d).balances) == total_balances(s.balances) + d.data.amount as int ;
+            }
+            else {
+                //assert updateDeposit(s,d).balances == s.balances + [d.data.amount];
+                distBalancesProp(s.balances,[d.data.amount]);
+                //assert total_balances(s.balances + [d.data.amount]) == total_balances(s.balances) + total_balances([d.data.amount]);
+            }
+        }
+    }
+
+
+    
+    lemma updateExistingBalance(s: BeaconState, index: ValidatorIndex, delta: Gwei)
+        requires index as int < |s.balances| 
+        requires s.balances[index] as int + delta as int < 0x10000000000000000
+        requires |s.balances| < VALIDATOR_REGISTRY_LIMIT as int
+
+        ensures total_balances(increase_balance(s,index,delta).balances) == total_balances(s.balances) + delta as int
+    {
+        //assert increase_balance(s,index,delta).balances[index] == s.balances[index] + delta;
+        //assert forall i :: 0 <= i < |s.balances| && i != index as int ==> increase_balance(s,index,delta).balances[i] == s.balances[i];
+
+        if index as int < |s.balances|-1 {
+            assert increase_balance(s,index,delta).balances == increase_balance(s,index,delta).balances[..index] + [increase_balance(s,index,delta).balances[index]] + increase_balance(s,index,delta).balances[(index+1)..];
+                                                                
+            //assert total_balances(increase_balance(s,index,delta).balances[..index]) == total_balances(s.balances[..index]);
+            //assert total_balances([increase_balance(s,index,delta).balances[index]]) == total_balances([s.balances[index]]) + delta as int;
+            //assert total_balances(increase_balance(s,index,delta).balances[(index+1)..]) == total_balances(s.balances[(index+1)..]);
+
+            //assert total_balances(increase_balance(s,index,delta).balances) == total_balances(increase_balance(s,index,delta).balances[..index] + [increase_balance(s,index,delta).balances[index]] + increase_balance(s,index,delta).balances[(index+1)..]);
+
+            distBalancesProp(increase_balance(s,index,delta).balances[..index], [increase_balance(s,index,delta).balances[index]]);
+            //assert total_balances(increase_balance(s,index,delta).balances[..index] + [increase_balance(s,index,delta).balances[index]]) == total_balances(increase_balance(s,index,delta).balances[..index]) + total_balances([increase_balance(s,index,delta).balances[index]]);
+            distBalancesProp(increase_balance(s,index,delta).balances[..index]+[increase_balance(s,index,delta).balances[index]], increase_balance(s,index,delta).balances[(index+1)..]);
+            //assert total_balances(increase_balance(s,index,delta).balances[..index] + [increase_balance(s,index,delta).balances[index]] + increase_balance(s,index,delta).balances[(index+1)..]) == total_balances(increase_balance(s,index,delta).balances[..index]) + total_balances([increase_balance(s,index,delta).balances[index]]) + total_balances(increase_balance(s,index,delta).balances[index+1..]);
+
+            //assert total_balances(increase_balance(s,index,delta).balances) == total_balances(increase_balance(s,index,delta).balances[..index]) + total_balances([increase_balance(s,index,delta).balances[index]]) + total_balances(increase_balance(s,index,delta).balances[index+1..]);
+            //assert total_balances(increase_balance(s,index,delta).balances) == total_balances(s.balances[..index]) + total_balances([s.balances[index]]) + delta as int + total_balances(s.balances[(index+1)..]);
+
+            //assert total_balances(increase_balance(s,index,delta).balances) == total_balances(s.balances[..index]) + total_balances([s.balances[index]]) + total_balances(s.balances[(index+1)..]) + delta as int;
+
+            assert s.balances == s.balances[..index] + [s.balances[index]] + s.balances[(index+1)..];
+            //assert total_balances(s.balances) == total_balances(s.balances[..index] + [s.balances[index]] + s.balances[(index+1)..]);
+
+            distBalancesProp(s.balances[..index], [s.balances[index]]);
+            //assert total_balances(s.balances[..index] + [s.balances[index]]) == total_balances(s.balances[..index]) + total_balances([s.balances[index]]);
+            distBalancesProp(s.balances[..index]+[s.balances[index]], s.balances[(index+1)..]);
+            //assert total_balances(s.balances[..index] + [s.balances[index]] + s.balances[(index+1)..]) == total_balances(s.balances[..index]) + total_balances([s.balances[index]]) + total_balances(s.balances[index+1..]);
+
+            //assert total_balances(increase_balance(s,index,delta).balances) == total_balances(s.balances) + delta as int;
+        }
+        else {
+            //assert index as int == |s.balances| - 1;
+            assert increase_balance(s,index,delta).balances == increase_balance(s,index,delta).balances[..index] + [increase_balance(s,index,delta).balances[index]];
+                                                                
+            //assert total_balances(increase_balance(s,index,delta).balances[..index]) == total_balances(s.balances[..index]);
+            //assert total_balances([increase_balance(s,index,delta).balances[index]]) == total_balances([s.balances[index]]) + delta as int;
+            
+            //assert total_balances(increase_balance(s,index,delta).balances) == total_balances(increase_balance(s,index,delta).balances[..index] + [increase_balance(s,index,delta).balances[index]]);
+
+            distBalancesProp(increase_balance(s,index,delta).balances[..index], [increase_balance(s,index,delta).balances[index]]);
+            //assert total_balances(increase_balance(s,index,delta).balances[..index] + [increase_balance(s,index,delta).balances[index]]) == total_balances(increase_balance(s,index,delta).balances[..index]) + total_balances([increase_balance(s,index,delta).balances[index]]);
+            
+            
+            //assert total_balances(increase_balance(s,index,delta).balances) == total_balances(s.balances[..index]) + total_balances([s.balances[index]]) + delta as int;
+
+            assert s.balances == s.balances[..index] + [s.balances[index]] ;
+            //assert total_balances(s.balances) == total_balances(s.balances[..index] + [s.balances[index]]);
+
+            distBalancesProp(s.balances[..index], [s.balances[index]]);
+            //assert total_balances(s.balances[..index] + [s.balances[index]]) == total_balances(s.balances[..index]) + total_balances([s.balances[index]]);
+            
+            //assert total_balances(increase_balance(s,index,delta).balances) == total_balances(s.balances) + delta as int;
+        }
+    }
+
+    lemma distBalancesProp(sb1: seq<Gwei>, sb2: seq<Gwei>)
+        ensures total_balances(sb1 + sb2) == total_balances(sb1) + total_balances(sb2) 
+    {
+        if |sb1| == 0 {
+            assert sb1 + sb2 == sb2;
+        }
+        else {
+            var sb := sb1 + sb2;
+            //assert sb == [sb1[0]] +  sb1[1..] + sb2;
+            assert sb[1..] == sb1[1..] + sb2;
+            assert total_balances(sb) == sb[0] as int + total_balances(sb[1..]);
+            //assert total_balances(sb1 + sb2) == sb[0] as int + total_balances(sb1[1..] + sb2);
+            distBalancesProp(sb1[1..],sb2);
+
+        }
+    }
+
+    lemma distDepositsProp(sd1: seq<Deposit>, sd2: seq<Deposit>)
+        ensures total_deposits(sd1 + sd2) == total_deposits(sd1) + total_deposits(sd2) 
+    {
+        if |sd2| == 0 {
+            assert sd1 + sd2 == sd1;
+        }
+        else {
+            var sd := sd1 + sd2;
+            //assert sd == sd1 + sd2[..|sd2|-1] +  [sd2[|sd2|-1]];
+            assert sd[..|sd|-1] == sd1 + sd2[..|sd2|-1] ;
+            assert total_deposits(sd) == total_deposits(sd[..|sd|-1]) + sd2[|sd2|-1].data.amount as int;
+            //assert total_deposits(sd1 + sd2) == total_deposits(sd1 + sd2[..|sd2|-1] ) + sd2[|sd2|-1].data.amount as int;
+            distDepositsProp(sd1, sd2[..|sd2|-1] );
+        }
+    }
+    lemma subsetDepositSumProp(deposits: seq<Deposit>, i: nat)
+        requires i <= |deposits|
+        ensures total_deposits(deposits[..i]) <= total_deposits(deposits);
+    {
+        if i == |deposits| {
+            assert deposits[..i] == deposits;
+        }
+        else {
+            //assert i < |deposits|;
+            assert deposits == deposits[..i] + deposits[i..];
+            assert total_deposits(deposits) == total_deposits(deposits[..i] + deposits[i..]);
+            distDepositsProp(deposits[..i], deposits[i..]);
+            //assert total_deposits(deposits[..i] + deposits[i..]) == total_deposits(deposits[..i]) + total_deposits(deposits[i..]); 
+        }
+    }
+
+
+
+
+
 }
