src/dafny/beacon/statetransition/ProcessOperations.p.dfy
@@ -44,8 +44,343 @@ module ProcessOperationsProofs {
     
     // Helper lemmas
 
+    lemma helperIndicesLemma(indices: seq<ValidatorIndex>)
+        requires |indices| > 0
+        ensures forall i :: 0 < i < |indices| ==> indices[..i+1] == indices[..i] + [indices[i]]
+    {
+        // Thanks Dafny
+    }
 
+    lemma helperIndicesLemma2(indices: seq<ValidatorIndex>)
+        requires |indices| > 0
+        ensures indices == indices[..|indices|-1] + [indices[|indices|-1]]
+    {
+        // Thanks Dafny
+    }
+
+    lemma helperIndicesLemma3(indices: seq<uint64>, i: nat)
+        requires 0 <= i < |indices|
+        ensures indices[..i+1] == indices[..i] + [indices[i]]
+    {
+        // Thanks Dafny
+    }
+
+    lemma helperIndicesLemma4(s: BeaconState, indices: seq<uint64>, i: nat)
+        requires 0 <= i <= |indices|
+        requires valid_state_indices(s, indices)
+        ensures valid_state_indices(s, indices[..i])
+    {
+        // Thanks Dafny
+    }
+
+    lemma helperIndicesLemma5(indices: seq<uint64>, i: nat)
+        requires i <= |indices|
+        ensures |indices[..i]| == i;
+    {
+        // Thanks Dafny
+    }
+
+    lemma helperIndicesLemma6(indices: seq<uint64>, i: nat)
+        requires i == |indices|
+        ensures indices[..i] == indices
+    {
+        // Thanks Dafny
+    }
+
+    lemma helperIndicesLemma7(indices: seq<uint64>, i: nat)
+        requires i < |indices|
+        ensures indices[..i+1] == indices[..i] + [indices[i]];
+    {
+        // Thanks Dafny
+    }
+
+
+
+///////////////////////////
+    lemma mappingPSIndices(ps: seq<ProposerSlashing>)
+        ensures forall i :: 0 <= i < |ps| ==> get_PS_validator_indices(ps)[i] == ps[i].header_1.proposer_index as int
+    {
+        //Thanks Dafny
+    }
+
+    lemma subsetMappingPSIndices(ps: seq<ProposerSlashing>, i : nat)
+        requires 0 <= i < |ps|
+        ensures get_PS_validator_indices(ps[..i]) == get_PS_validator_indices(ps)[..i]
+    {
+        if |ps| == 0 {}
+        else {
+            assert ps == ps[..i] + ps[i..];
+            
+            mappingPSIndices(ps[..i]);
+            assert forall j :: 0 <= j < |ps[..i]| ==> get_PS_validator_indices(ps[..i])[j] == ps[j].header_1.proposer_index as int;
+
+            mappingPSIndices(ps);
+            assert forall j :: 0 <= j < |ps| ==> get_PS_validator_indices(ps)[j] == ps[j].header_1.proposer_index as int;
+        }
+    }
+
+    lemma helperPSLemma(s: BeaconState, ps: ProposerSlashing)
+        requires ps.header_1.slot == ps.header_2.slot
+        requires ps.header_1.proposer_index == ps.header_2.proposer_index 
+        requires ps.header_1 == ps.header_2
+        requires ps.header_1.proposer_index as int < |s.validators| 
+
+        // requires is_active_validator: (!v.slashed) && (v.activation_epoch <= epoch < v.withdrawable_epoch)
+        requires !s.validators[ps.header_1.proposer_index].slashed
+        requires s.validators[ps.header_1.proposer_index].activation_epoch <= get_current_epoch(s) < s.validators[ps.header_1.proposer_index].withdrawable_epoch
+ 
+        requires |get_active_validator_indices(s.validators, get_current_epoch(s))| > 0
+        requires |s.validators| == |s.balances|
+        
+        ensures forall i :: 0 <= i < |s.validators| && i != ps.header_1.proposer_index as int ==> updateProposerSlashing(s, ps).validators[i].exitEpoch == s.validators[i].exitEpoch
+        ensures forall i :: 0 <= i < |s.validators| && i != ps.header_1.proposer_index as int ==> updateProposerSlashing(s, ps).validators[i].slashed == s.validators[i].slashed
+        ensures forall i :: 0 <= i < |s.validators| && i != ps.header_1.proposer_index as int ==> updateProposerSlashing(s, ps).validators[i].withdrawable_epoch == s.validators[i].withdrawable_epoch
+    {
+        // Thanks Dafny
+    }
+
+    lemma helperPSLemma2(s: BeaconState, ps: seq<ProposerSlashing>)
+        requires  |get_PS_validator_indices(ps)| > 0
+        requires forall i :: i in get_PS_validator_indices(ps) ==> 0 <= i < |s.validators| 
+        requires forall i :: i in get_PS_validator_indices(ps) ==> !s.validators[i].slashed
+        requires forall i :: i in get_PS_validator_indices(ps) ==> s.validators[i].activation_epoch <= get_current_epoch(s) < s.validators[i].withdrawable_epoch
+        
+
+        ensures forall i :: i in get_PS_validator_indices(ps[..|ps|-1]) ==> 0 <= i < |s.validators|
+        ensures forall i :: i in get_PS_validator_indices(ps[..|ps|-1]) ==> !s.validators[i].slashed
+        ensures forall i :: i in get_PS_validator_indices(ps[..|ps|-1]) ==> s.validators[i].activation_epoch <= get_current_epoch(s) < s.validators[i].withdrawable_epoch
+    {
+        mappingPSIndices(ps);
+        assert forall i :: 0 <= i < |ps| ==> get_PS_validator_indices(ps)[i] == ps[i].header_1.proposer_index as int;
+
+        subsetMappingPSIndices(ps, |ps|-1);
+        assert get_PS_validator_indices(ps[..|ps|-1]) == get_PS_validator_indices(ps)[..|ps|-1];
+        
+        assert forall i :: i in get_PS_validator_indices(ps) ==> 0 <= i < |s.validators|; // from requires
+        assert forall i :: 0 <= i < |ps| ==> get_PS_validator_indices(ps)[i] == ps[i].header_1.proposer_index as int;
+        assert forall i :: 0 <= i < |ps| ==> ps[i].header_1.proposer_index as int in get_PS_validator_indices(ps) ;
+        
+    }
+
+
+    lemma updateProposerSlashingLemma(s: BeaconState, ps : ProposerSlashing)
+        requires ps.header_1.slot == ps.header_2.slot
+        requires ps.header_1.proposer_index == ps.header_2.proposer_index 
+        requires ps.header_1 == ps.header_2
+        requires ps.header_1.proposer_index as int < |s.validators| 
+        //requires is_slashable_validator(s.validators[ps.header_1.proposer_index], get_current_epoch(s));
+        //(!v.slashed) && (v.activation_epoch <= epoch < v.withdrawable_epoch)
+        requires !s.validators[ps.header_1.proposer_index].slashed
+        requires s.validators[ps.header_1.proposer_index].activation_epoch <= get_current_epoch(s) < s.validators[ps.header_1.proposer_index].withdrawable_epoch
+        
+        requires |get_active_validator_indices(s.validators, get_current_epoch(s))| > 0
+        requires |s.validators| == |s.balances|
+        
+        ensures |get_active_validator_indices(updateProposerSlashing(s, ps).validators, get_current_epoch(s))| > 0
+    {
+        var index := ps.header_1.proposer_index; // validator to be slashed
+        var slashable_validator := s.validators[index];
+        var epoch : Epoch := get_current_epoch(s);
+
+        assert updateProposerSlashing(s, ps) == slash_validator(s, ps.header_1.proposer_index, get_beacon_proposer_index(s));
+        slashValidatorPreservesActivateValidators(s, ps.header_1.proposer_index, get_beacon_proposer_index(s));
+        assert |get_active_validator_indices(updateProposerSlashing(s, ps).validators, get_current_epoch(s))| > 0;
+
+    }
+
+    lemma helperPSLemma3(s: BeaconState, ps : seq<ProposerSlashing>)
+        requires forall i :: 0 <= i < |ps| ==> ps[i].header_1.proposer_index as int < |s.validators| 
+        requires forall i :: 0 <= i < |ps| ==> !s.validators[ps[i].header_1.proposer_index].slashed 
+        requires forall i :: 0 <= i < |ps| ==> s.validators[ps[i].header_1.proposer_index].activation_epoch <= get_current_epoch(s) < s.validators[ps[i].header_1.proposer_index].withdrawable_epoch
+
+        ensures forall i :: i in get_PS_validator_indices(ps) ==> 0 <= i < |s.validators|
+        ensures forall i :: i in get_PS_validator_indices(ps) ==> !s.validators[i].slashed
+        ensures forall i :: i in get_PS_validator_indices(ps) ==> s.validators[i].activation_epoch <= get_current_epoch(s) < s.validators[i].withdrawable_epoch
+    {
+        // Thanks Dafny
+    }
+
+    lemma helperPSLemma4(ps : seq<ProposerSlashing>)
+        requires |ps| > 0
+        requires forall i,j :: 0 <= i < j < |ps| && i != j ==> ps[i].header_1.proposer_index!= ps[j].header_1.proposer_index // ve indices are unique
+        ensures ps[|ps|-1].header_1.proposer_index as int !in get_PS_validator_indices(ps[..|ps|-1])
+    {
+        mappingPSIndices(ps[..|ps|-1]);
+        assert forall i :: 0 <= i < |ps[..|ps|-1]| ==> get_PS_validator_indices(ps[..|ps|-1])[i] == ps[i].header_1.proposer_index as int;
+    }
+
+    lemma helperPSLemma5(s: BeaconState, ps : seq<ProposerSlashing>)
+        requires |ps| > 0
+        requires forall i,j :: 0 <= i < j < |ps| && i != j ==> ps[i].header_1.proposer_index!= ps[j].header_1.proposer_index // ve indices are unique
+        requires forall i :: 0 <= i < |ps| ==> ps[i].header_1.slot == ps[i].header_2.slot
+        requires forall i :: 0 <= i < |ps| ==> ps[i].header_1.proposer_index == ps[i].header_2.proposer_index 
+        requires forall i :: 0 <= i < |ps| ==> ps[i].header_1 == ps[i].header_2
+        requires forall i :: 0 <= i < |ps| ==> ps[i].header_1.proposer_index as int < |s.validators| 
+        requires forall i :: 0 <= i < |ps| ==> !s.validators[ps[i].header_1.proposer_index].slashed 
+        requires forall i :: 0 <= i < |ps| ==> s.validators[ps[i].header_1.proposer_index].activation_epoch <= get_current_epoch(s) < s.validators[ps[i].header_1.proposer_index].withdrawable_epoch
+
+        ensures forall i,j :: 0 <= i < j < |ps[..|ps|-1]| && i != j ==> ps[i].header_1.proposer_index!= ps[j].header_1.proposer_index
+        ensures forall i :: 0 <= i < |ps[..|ps|-1]| ==> ps[i].header_1.slot == ps[i].header_2.slot;
+        ensures forall i :: 0 <= i < |ps[..|ps|-1]| ==> ps[i].header_1.proposer_index == ps[i].header_2.proposer_index ;
+        ensures forall i :: 0 <= i < |ps[..|ps|-1]| ==> ps[i].header_1 == ps[i].header_2;
+        ensures forall i :: 0 <= i < |ps[..|ps|-1]| ==> ps[i].header_1.proposer_index as int < |s.validators| ;
+        ensures forall i :: 0 <= i < |ps[..|ps|-1]| ==> !s.validators[ps[i].header_1.proposer_index].slashed ;
+        ensures forall i :: 0 <= i < |ps[..|ps|-1]| ==> s.validators[ps[i].header_1.proposer_index].activation_epoch <= get_current_epoch(s) < s.validators[ps[i].header_1.proposer_index].withdrawable_epoch;
+           
+    {
+    }
+
+    lemma helperPSLemma6(ps : seq<ProposerSlashing>)
+        requires |ps| > 0
+        ensures get_PS_validator_indices(ps[..|ps|-1]) + [ps[|ps|-1].header_1.proposer_index as int] == get_PS_validator_indices(ps)
+        ensures forall i : int :: i !in get_PS_validator_indices(ps[..|ps|-1]) && i != ps[|ps|-1].header_1.proposer_index as int ==>
+                i !in get_PS_validator_indices(ps)
+    {
+        mappingPSIndices(ps);
+        subsetMappingPSIndices(ps, |ps|-1);
+    }
+
+
+    ///////////////
+
+    lemma AttestationHelperLemma(s: BeaconState, s1: BeaconState, a: Attestation)
+        requires attestationIsWellFormed(s, a);
+        requires s1.validators == s.validators
+        requires s1.slot == s.slot
+        requires s1.current_justified_checkpoint == s.current_justified_checkpoint
+        requires s1.previous_justified_checkpoint == s.previous_justified_checkpoint
+        ensures attestationIsWellFormed(s1, a);
+    { // Thanks Dafny
+    }
+
+    //////////////////
+
+    lemma VolExitLemma1(s: BeaconState, voluntary_exit: VoluntaryExit)
+        requires |s.validators| == |s.balances|
+        requires voluntary_exit.validator_index as int < |s.validators| 
+        requires minimumActiveValidators(s)
+        
+        requires !s.validators[voluntary_exit.validator_index].slashed
+        requires s.validators[voluntary_exit.validator_index].activation_epoch <= get_current_epoch(s) < s.validators[voluntary_exit.validator_index].withdrawable_epoch
+
+        requires s.validators[voluntary_exit.validator_index].exitEpoch == FAR_FUTURE_EPOCH
+        requires get_current_epoch(s) >= voluntary_exit.epoch
+        requires get_current_epoch(s) >= s.validators[voluntary_exit.validator_index].activation_epoch + SHARD_COMMITTEE_PERIOD 
+
+        ensures minimumActiveValidators(updateVoluntaryExit(s, voluntary_exit))
+    {
+        // var s1 := updateVoluntaryExit(s, voluntary_exit);
+        // assert get_current_epoch(s) == get_current_epoch(s1);
+        // assert exists v :: 0 <= v < |s.validators| && s.validators[v].activation_epoch <= get_current_epoch(s) < s.validators[v].exitEpoch;
+        // assert forall v :: 0 <= v < |s.validators| ==> s.validators[v].activation_epoch <= get_current_epoch(s) < s.validators[v].exitEpoch
+        //                                             ==> s1.validators[v].activation_epoch <= get_current_epoch(s1) < s1.validators[v].exitEpoch;
+        // assert exists v :: 0 <= v < |s1.validators| && s1.validators[v].activation_epoch <= get_current_epoch(s1) < s1.validators[v].exitEpoch;
+        // assert exists v :: 0 <= v < |s1.validators| && is_active_validator(s1.validators[v], get_current_epoch(s1));
+        // assert |get_active_validator_indices(s1.validators, get_current_epoch(s1))| > 0 ==> 
+        //     (exists v :: 0 <= v < |s1.validators| && is_active_validator(s1.validators[v], get_current_epoch(s1)));
+        // assert  minimumActiveValidators(s1);
+    }
+
+
+    lemma helperVoluntaryExitLemma3(s: BeaconState, ve: seq<VoluntaryExit>)
+        requires forall i :: 0 <= i < |ve| ==> ve[i].validator_index as int < |s.validators| 
+        //requires forall i :: 0 <= i < |ve| ==> is_active_validator(s.validators[ve[i].validator_index], get_current_epoch(s))
+        requires forall i :: 0 <= i < |ve| ==> !s.validators[ve[i].validator_index].slashed
+        requires forall i :: 0 <= i < |ve| ==> s.validators[ve[i].validator_index].activation_epoch <= get_current_epoch(s) < s.validators[ve[i].validator_index].withdrawable_epoch
+
+        requires forall i :: 0 <= i < |ve| ==> s.validators[ve[i].validator_index].exitEpoch == FAR_FUTURE_EPOCH
+        requires forall i :: 0 <= i < |ve| ==> get_current_epoch(s) >= s.validators[ve[i].validator_index].activation_epoch + SHARD_COMMITTEE_PERIOD 
+
+        ensures forall i :: i in get_VolExit_validator_indices(ve) ==> 0 <= i < |s.validators| 
+        
+        //ensures forall i :: i in get_VolExit_validator_indices(ve) ==> is_active_validator(s.validators[i], get_current_epoch(s))
+        ensures forall i :: i in get_VolExit_validator_indices(ve) ==> !s.validators[i].slashed
+        ensures forall i :: i in get_VolExit_validator_indices(ve) ==> s.validators[i].activation_epoch <= get_current_epoch(s) < s.validators[i].withdrawable_epoch
+
+        ensures forall i :: i in get_VolExit_validator_indices(ve) ==> s.validators[i].exitEpoch == FAR_FUTURE_EPOCH
+        ensures forall i :: i in get_VolExit_validator_indices(ve) ==> get_current_epoch(s) >= s.validators[i].activation_epoch + SHARD_COMMITTEE_PERIOD 
+    {
+        // Thanks Dafny
+    }
+
+    lemma helperVoluntaryExitLemma2(s: BeaconState, ve: seq<VoluntaryExit>)
+        requires  |get_VolExit_validator_indices(ve)| > 0
+        requires forall i :: i in get_VolExit_validator_indices(ve) ==> 0 <= i < |s.validators| 
+        requires forall i :: i in get_VolExit_validator_indices(ve) ==> !s.validators[i].slashed
+        requires forall i :: i in get_VolExit_validator_indices(ve) ==> s.validators[i].activation_epoch <= get_current_epoch(s) < s.validators[i].withdrawable_epoch
+        requires forall i :: i in get_VolExit_validator_indices(ve) ==> s.validators[i].exitEpoch == FAR_FUTURE_EPOCH
+        requires forall i :: i in get_VolExit_validator_indices(ve) ==> get_current_epoch(s) >= s.validators[i].activation_epoch + SHARD_COMMITTEE_PERIOD 
     
+
+        ensures forall i :: i in get_VolExit_validator_indices(ve[..|ve|-1]) ==> 0 <= i < |s.validators|
+        ensures forall i :: i in get_VolExit_validator_indices(ve[..|ve|-1]) ==> !s.validators[i].slashed
+        ensures forall i :: i in get_VolExit_validator_indices(ve[..|ve|-1]) ==> s.validators[i].activation_epoch <= get_current_epoch(s) < s.validators[i].withdrawable_epoch
+        ensures forall i :: i in get_VolExit_validator_indices(ve[..|ve|-1]) ==> s.validators[i].exitEpoch == FAR_FUTURE_EPOCH
+        ensures forall i :: i in get_VolExit_validator_indices(ve[..|ve|-1]) ==> get_current_epoch(s) >= s.validators[i].activation_epoch + SHARD_COMMITTEE_PERIOD
+    {
+        mappingVolExitIndices(ve);
+        assert forall i :: 0 <= i < |ve| ==> get_VolExit_validator_indices(ve)[i] == ve[i].validator_index as int;
+
+        subsetMappingVolExitIndices(ve, |ve|-1);
+        assert get_VolExit_validator_indices(ve[..|ve|-1]) == get_VolExit_validator_indices(ve)[..|ve|-1];
+        
+        assert forall i :: i in get_VolExit_validator_indices(ve) ==> 0 <= i < |s.validators|; // from requires
+        assert forall i :: 0 <= i < |ve| ==> get_VolExit_validator_indices(ve)[i] == ve[i].validator_index as int;
+        assert forall i :: 0 <= i < |ve| ==> ve[i].validator_index as int in get_VolExit_validator_indices(ve) ;
+        
+    }
+
+    lemma helperVoluntaryExitLemma(s: BeaconState, exit: VoluntaryExit)
+        requires |s.validators| == |s.balances|
+        requires exit.validator_index as int < |s.validators| 
+        // requires is_active_validator(s.validators[voluntary_exit.validator_index], get_current_epoch(s))
+        // (!v.slashed) && (v.activation_epoch <= epoch < v.withdrawable_epoch)
+        requires !s.validators[exit.validator_index].slashed
+        requires s.validators[exit.validator_index].activation_epoch <= get_current_epoch(s) < s.validators[exit.validator_index].withdrawable_epoch
+
+        requires s.validators[exit.validator_index].exitEpoch == FAR_FUTURE_EPOCH
+        requires get_current_epoch(s) >= exit.epoch
+        requires get_current_epoch(s) >= s.validators[exit.validator_index].activation_epoch + SHARD_COMMITTEE_PERIOD 
+        
+        ensures forall i :: 0 <= i < |s.validators| && i != exit.validator_index as int ==> updateVoluntaryExit(s, exit).validators[i].exitEpoch == s.validators[i].exitEpoch
+        ensures forall i :: 0 <= i < |s.validators| && i != exit.validator_index as int ==> updateVoluntaryExit(s, exit).validators[i].slashed == s.validators[i].slashed
+        ensures forall i :: 0 <= i < |s.validators| && i != exit.validator_index as int ==> updateVoluntaryExit(s, exit).validators[i].withdrawable_epoch == s.validators[i].withdrawable_epoch
+    {
+        // Thanks Dafny
+    }
+
+    lemma mappingVolExitIndices(ve: seq<VoluntaryExit>)
+        ensures forall i :: 0 <= i < |ve| ==> get_VolExit_validator_indices(ve)[i] == ve[i].validator_index as int
+    {
+        //Thanks Dafny
+    }
+
+    lemma subsetMappingVolExitIndices(ve: seq<VoluntaryExit>, i : nat)
+        requires 0 <= i < |ve|
+        ensures get_VolExit_validator_indices(ve[..i]) == get_VolExit_validator_indices(ve)[..i]
+    {
+        if |ve| == 0 {}
+        else {
+            assert ve == ve[..i] + ve[i..];
+            
+            mappingVolExitIndices(ve[..i]);
+            assert forall j :: 0 <= j < |ve[..i]| ==> get_VolExit_validator_indices(ve[..i])[j] == ve[j].validator_index as int;
+
+            mappingVolExitIndices(ve);
+            assert forall j :: 0 <= j < |ve| ==> get_VolExit_validator_indices(ve)[j] == ve[j].validator_index as int;
+        }
+    }
+
+    //lemma PSpreconditionLemma()
+    lemma helperVolExitLemma4(ve : seq<VoluntaryExit>)
+        requires |ve| > 0
+        requires forall i,j :: 0 <= i < j < |ve| && i != j ==> ve[i].validator_index!= ve[j].validator_index // ve indices are unique
+        ensures ve[|ve|-1].validator_index as int !in get_VolExit_validator_indices(ve[..|ve|-1])
+    {
+        mappingVolExitIndices(ve[..|ve|-1]);
+        assert forall i :: 0 <= i < |ve[..|ve|-1]| ==> get_VolExit_validator_indices(ve[..|ve|-1])[i] == ve[i].validator_index as int;
+    }
+
     
 
 }
